they work

applicationwebsite.bpl
@@ -1,46 +1,183 @@
+
+type MapIntCollege = [int] Ref;
+
+// Each ApplicationWebsite will have its own map of college.
+
+var mapOfColleges : [Ref]MapIntCollege; 
+
+var maxSize : [Ref]int;
+
 // Each ApplicationWebsite has its own map of college
-// I use mapOfColleges from mapcollege.bpl
-//var mapOfAvailableColleges : [Ref]MapIntCollege;
 
 var packedApplicationWebsiteField : [Ref]bool;
 var fracApplicationWebsiteField : [Ref]real;
 
 procedure PackApplicationWebsiteField(m: MapIntCollege, this:Ref);
-requires (packedApplicationWebsiteField[this]==false) &&
- 	(mapOfColleges[this] == m); 
+requires (packedApplicationWebsiteField[this]==false);
+requires (mapOfColleges[this] == m); 
+// TODO add something about params, the values can be null or not
+requires  (forall j:int :: (  ((j<=maxSize[this]) && (j>=0)) ==> 
+           packedKeyValuePair[this, j] && (fracKeyValuePair[this, j] > 0.0) ) );
 
 procedure UnpackApplicationWebsiteField(m: MapIntCollege, this:Ref);
 requires packedApplicationWebsiteField[this];
 requires fracApplicationWebsiteField[this] > 0.0;
-ensures	(mapOfColleges[this] == m); 
+ensures	(mapOfColleges[this] == m);
+// TODO add something about params, the values can be null or not
+ensures  (forall j:int :: (  ((j<=maxSize[this]) && (j>=0)) ==> 
+           packedKeyValuePair[this, j] && (fracKeyValuePair[this, j] > 0.0) ) );
 
-procedure submitApplicationGetCollege(int collegeNumber) returns (r: Ref)
-modifies mapOfColleges;
-requires packedApplicationWebsiteField[this] && 
-	(fracApplicationWebsiteField[this] > 0.0);
-ensures ( packedCollegeBuildingsFew[result] && 
-	(fracCollegeBuildingsFew[result] > 0.0) ) ||
-	( packedCollegeBuildingsMany[result] &&
-	(fracCollegeBuildingsMany[result] > 0.0) );
+// the type of packed and frac is different here because 
+// we are dealing with maps and they have an extra index, the key, 
+// that we need in order to get to the value.
+var packedKeyValuePair : [Ref, int]bool;
+var fracKeyValuePair : [Ref, int]real;
+
+procedure PackKeyValuePair(m:MapIntCollege, key:int, value:Ref, this:Ref);
+requires packedKeyValuePair[this, key] == false;
+requires mapOfColleges[this] == m;
+requires  (m[key] == value);
+
+procedure UnpackKeyValuePair(m:MapIntCollege, key:int, value:Ref, this:Ref);
+requires packedKeyValuePair[this, key];
+requires fracKeyValuePair[this, key] > 0.0;
+ensures (mapOfColleges[this] == m);
+ensures (m[key] == value);
+
+procedure createMapCollege(maxSize1:int, this: Ref)
+modifies maxSize, mapOfColleges, packedKeyValuePair, fracKeyValuePair;
+requires (maxSize1>=0);
+// TODO add something about param being null in the ensures below
+ensures (forall j:int :: ((j<=maxSize1) && (j>=0)) ==> (packedKeyValuePair[this, j] && (fracKeyValuePair[this, j]==1.0)) ) ;
+ensures maxSize[this] == maxSize1;
 {
-	var college : Ref;
-	call college := lookup(collegeNumber, mapOfColleges[this]);
-	// might be able to say var r : Ref from the beginning
-	r := college;
+call makeMapNull(maxSize1, this);
+maxSize[this] := maxSize1;
 }
 
-procedure main(this:Ref) 
-modifies mapOfColleges;
+procedure makeMapNull(i : int, this:Ref)
+modifies mapOfColleges, packedKeyValuePair, fracKeyValuePair;
+requires (i>=0);
+ensures (forall j:int :: (((j<=i) && (j>=0) ) ==> (packedKeyValuePair[this, j] && ( fracKeyValuePair[this, j] == 1.0 )))  );
+{
+if (i==0) {
+	mapOfColleges[this][i] := null;	
+  	packedKeyValuePair[this, i] := true;
+  	fracKeyValuePair[this, i] := 1.0;
+} else if (i>0) {
+	call makeMapNull(i-1, this);
+  	mapOfColleges[this][i] := null;	
+  	packedKeyValuePair[this, i] := true;
+  	fracKeyValuePair[this, i] := 1.0;
+}
+}
+
+procedure containsKey(key1: int, this:Ref) returns (b:bool)
+requires packedApplicationWebsiteField[this];
+requires (fracApplicationWebsiteField[this] > 0.0);
+//requires this#k MapOfCollegesField()
+//ensures (b == true) && (exists c:College ==> (this#k KeyValuePair(key1, c))	 ||
+//	(b == false) && (this#k KeyValuePair(key1, null)) 
+{
+	b := true;
+	if (mapOfColleges[this][key1] == null) {
+		b := false;	
+	} 
+}
+	
+procedure put(key1 : int, college1: Ref, this:Ref) 
+modifies mapOfColleges, packedKeyValuePair;
+requires packedApplicationWebsiteField[this]==false;
+requires (fracApplicationWebsiteField[this] > 0.0);
+// This put procedure will be called with null for the value in packedKeyValuePair.
+requires packedKeyValuePair[this, key1];
+requires (fracKeyValuePair[this, key1] > 0.0);
+ensures packedKeyValuePair[this, key1];
+ensures	(fracKeyValuePair[this, key1] > 0.0);
+{
+  call UnpackKeyValuePair(mapOfColleges[this], key1, null, this);
+  packedKeyValuePair[this, key1] := false;
+	mapOfColleges[this][key1] := college1;	
+  call PackKeyValuePair(mapOfColleges[this], key1, college1, this);
+  packedKeyValuePair[this, key1] := true;
+}
+	
+procedure get(key1:int, this:Ref) returns (c:Ref)
+requires packedKeyValuePair[this, key1];
+requires	(fracKeyValuePair[this, key1] > 0.0);
+ensures packedKeyValuePair[this, key1];
+ensures	(fracKeyValuePair[this, key1] > 0.0);
+//requires this#k MapOfCollegesField()
+//ensures this#k KeyValuePair(key1, result)
+{
+	c := mapOfColleges[this][key1];
+}
+	
+procedure lookup(collegeNumber:int, this:Ref) returns (r:Ref)
+modifies mapOfColleges, packedCollegeFields, fracCollegeFields,collegeNumber,
+       endowment, packedKeyValuePair, packedApplicationWebsiteField;
+requires (collegeNumber<=maxSize[this]) && (0<=collegeNumber);
+requires packedApplicationWebsiteField[this];
+requires (fracApplicationWebsiteField[this] > 0.0);
+ensures packedKeyValuePair[this, collegeNumber];
+ensures	(fracKeyValuePair[this, collegeNumber] > 0.0);
+//ensures this#k KeyValuePair(collegeNumber, result)
+{
+var temp:bool;
+var c:Ref;
+call temp := containsKey(collegeNumber, this);
+call UnpackApplicationWebsiteField(mapOfColleges[this], this);
+packedApplicationWebsiteField[this]:=false;
+if (temp == false) 
+	{
+		call ConstructCollege(collegeNumber, c);
+		packedCollegeFields[c] := false;
+		call PackCollegeFields(collegeNumber, c);
+		packedCollegeFields[c] := true;
+		fracCollegeFields[c] := 1.0;
+    
+		call put(collegeNumber, c, this);
+	}
+call r:= get(collegeNumber, this);
+}
+
+procedure ConstructApplicationWebsite(maxSize1:int, this:Ref)
+modifies maxSize, mapOfColleges, packedKeyValuePair, fracKeyValuePair;
+requires (maxSize1>=0);
+ensures (forall j:int :: ((j<=maxSize1) && (j>=0)) ==> (packedKeyValuePair[this, j] && (fracKeyValuePair[this, j]==1.0)) ) ;
+ensures maxSize[this] == maxSize1;
+{
+	call createMapCollege(maxSize1, this);
+ }
+
+procedure submitApplicationGetCollege(collegeNumber:int, this:Ref) returns (r: Ref)
+modifies mapOfColleges, packedCollegeFields, fracCollegeFields, collegeNumber, endowment,
+        packedKeyValuePair, packedApplicationWebsiteField;
+requires packedApplicationWebsiteField[this];
+requires (fracApplicationWebsiteField[this] > 0.0);
+requires (collegeNumber<=maxSize[this]) && (0<=collegeNumber);
+{
+	call r := lookup(collegeNumber, this);
+}
+
+procedure main1(this:Ref) 
+modifies mapOfColleges, packedApplicationWebsiteField,
+  packedStudentAppFacilitiesFew, packedStudentAppFacilitiesMany,
+  packedCollegeFields, fracCollegeFields, collegeNumber, endowment,
+  fracApplicationWebsiteField, college, facilities, campusNumber, 
+  fracMultipleOf, packedMultipleOf, fracStudentAppFacilitiesFew,
+  fracStudentAppFacilitiesMany, maxSize, divider, value,
+  fracCollegeFacilitiesFew, fracCollegeFacilitiesMany,
+  packedKeyValuePair, fracKeyValuePair,
+        packedCollegeFacilitiesFew, packedCollegeFacilitiesMany;
 {
 	var website : Ref;
-	var college, college2 : Ref;
-	var app1, app2 : Ref;
-	var app3, app4 : Ref;
-	assume (college != college2);
+	var college : Ref;
+	var app1, app2: Ref;
+  	var tempbo : bool;
 	assume (app1 != app2);
-	assume (app3 != app4);
 	
-	call ConstructApplicationWebsite(5, website);
+	call ConstructApplicationWebsite(100, website);
 	packedApplicationWebsiteField[website] := false;
 	call PackApplicationWebsiteField(mapOfColleges[website], website);
 	packedApplicationWebsiteField[website] := true;
@@ -62,12 +199,36 @@ modifies mapOfColleges;
 	fracStudentAppFacilitiesFew[app2] := 1.0;
 	fracCollegeFacilitiesFew[college] := fracCollegeFacilitiesFew[college] / 2.0;
 
-	call checkFewFacilities(app1);
+	call tempbo := checkFacilitiesFew(app1);
 	call changeApplicationFew(34, app1);
-	call checkFewFacilities(app2);
+	call tempbo := checkFacilitiesFew(app2);
+}
 
-	// ---- code below this is similar to above
+// ---- procedure below is similar to above
 
+procedure main2(this:Ref) 
+modifies mapOfColleges, packedApplicationWebsiteField,
+  packedStudentAppFacilitiesFew, packedStudentAppFacilitiesMany,
+  packedCollegeFields, fracCollegeFields, collegeNumber, endowment,
+  fracApplicationWebsiteField, college, facilities, campusNumber, 
+  fracMultipleOf, packedMultipleOf, fracStudentAppFacilitiesFew,
+  fracStudentAppFacilitiesMany, maxSize, divider, value,
+  fracCollegeFacilitiesFew, fracCollegeFacilitiesMany,
+  packedKeyValuePair, fracKeyValuePair,
+        packedCollegeFacilitiesFew, packedCollegeFacilitiesMany;
+{
+	var website : Ref;
+	var college2 : Ref;
+	var app3, app4 : Ref;
+  	var tempbo : bool;
+	assume (app3 != app4);
+  
+  	call ConstructApplicationWebsite(100, website);
+	packedApplicationWebsiteField[website] := false;
+	call PackApplicationWebsiteField(mapOfColleges[website], website);
+	packedApplicationWebsiteField[website] := true;
+	fracApplicationWebsiteField[website] := 1.0;
+  
 	call college2 := submitApplicationGetCollege(56, website);
 
 	call ConstructStudentApplication(college2, 45, app3);
@@ -75,7 +236,7 @@ modifies mapOfColleges;
 	call PackStudentAppFacilitiesMany(college2, 45, app3);
 	packedStudentAppFacilitiesMany[app3] := true;
 	fracStudentAppFacilitiesMany[app3] := 1.0;
-	fracCollegeFacilitiesMany[college] := fracCollegeFacilitiesMany[college2] / 2.0;
+	fracCollegeFacilitiesMany[college2] := fracCollegeFacilitiesMany[college2] / 2.0;
 
 	call ConstructStudentApplication(college2, 97, app4);
 	packedStudentAppFacilitiesMany[app4] := false;
@@ -84,7 +245,7 @@ modifies mapOfColleges;
 	fracStudentAppFacilitiesMany[app4] := 1.0;
 	fracCollegeFacilitiesMany[college2] := fracCollegeFacilitiesMany[college2] / 2.0;
 
-	call checkFewFacilities(app3);
-	call changeApplicationFew(78, app3);
-	call checkFewFacilities(app4);
+	call tempbo := checkFacilitiesMany(app3);
+	call changeApplicationMany(78, app3);
+	call tempbo := checkFacilitiesMany(app4);
 }
