intcell.bpl
@@ -1,28 +1,20 @@
+//intcell.bpl
 type Ref;
 const null: Ref;
 
 var value: [Ref]int;
+var divider : [Ref]int;
 var packedMultipleOf: [Ref] bool;
 var fracMultipleOf: [Ref] real;
 
-var packedMultipleOf21: [Ref] bool;
-var fracMultipleOf21: [Ref] real;
+var packedBasicIntCell: [Ref] bool;
+var fracBasicIntCell: [Ref] real;
 
-var packedMultipleOf16: [Ref] bool;
-var fracMultipleOf16: [Ref] real;
+var packedIntCellMany : [Ref] bool;
+var fracIntCellMany : [Ref]real;
 
-var packedMultipleOf15: [Ref] bool;
-var fracMultipleOf15: [Ref] real;
-
-var packedMultipleOf14: [Ref] bool;
-var fracMultipleOf14: [Ref] real;
-
-var packedMultipleOf33: [Ref] bool;
-var fracMultipleOf33: [Ref] real;
-
-var packedMultipleOf4: [Ref] bool;
-var fracMultipleOf4: [Ref] real;
-
+var packedIntCellFew : [Ref] bool;
+var fracIntCellFew : [Ref]real;
 
 function modulo(x:int, y:int) returns (int);
 axiom (forall x:int, y:int :: {modulo(x,y)} 
@@ -35,81 +27,67 @@ axiom (forall x:int, y:int :: {modulo(x,y)}
     ((x <= 0) &&(y < 0) ==> (y <= modulo(x,y) ) && (modulo(x,y) <= 0) )
    ); 
 
-// TODO maybe need to add a field value that holds a, the one we divide by
+procedure PackBasicIntCell(a: int, v:int, this:Ref);
+requires (packedBasicIntCell[this]==false);
+requires (value[this] == v);
+requires (divider[this] == a);
+
+procedure UnpackBasicIntCell(a: int, v:int, this:Ref);
+requires packedBasicIntCell[this];
+requires fracBasicIntCell[this] > 0.0;
+ensures	(value[this] == v);
+ensures (divider[this] == a);
+
 procedure PackMultipleOf(a: int, v:int, this:Ref);
-requires (packedMultipleOf[this]==false) &&
- 	(value[this] == v) && (modulo(v,a) == 0); 
+requires (packedMultipleOf[this]==false);
+requires (value[this] == v);
+requires (divider[this] == a);
+requires ( (v - int(v/a)*a )==0);
 
 procedure UnpackMultipleOf(a: int, v:int, this:Ref);
 requires packedMultipleOf[this];
 requires fracMultipleOf[this] > 0.0;
-ensures	(value[this] == v) && (modulo(v,a) == 0); 
+ensures	(value[this] == v);
+ensures (divider[this] == a);
+ensures	 ( (v - int(v/a)*a )==0);
 
-procedure PackMultipleOf21(v:int, this:Ref);
-requires (packedMultipleOf21[this]==false) &&
- 	(value[this] == v) && (modulo(v,21) == 0); 
+procedure PackIntCellMany(divi: int, val:int, quot:int, this:Ref);
+requires (packedIntCellMany[this]==false);
+requires (value[this] == val);
+requires (divider[this] == divi);
+requires (quot >= 10);
 
-procedure UnpackMultipleOf21(v:int, this:Ref);
-requires packedMultipleOf21[this];
-requires fracMultipleOf21[this] > 0.0;
-ensures	(value[this] == v) && (modulo(v,21) == 0); 
+procedure UnpackIntCellMany(divi: int, val:int, quot:int, this:Ref);
+requires packedIntCellMany[this];
+requires fracIntCellMany[this] > 0.0;
+ensures	(value[this] == val);
+ensures (divider[this] == divi);
+ensures (quot >= 10);
 
-procedure PackMultipleOf16(v:int, this:Ref);
-requires (packedMultipleOf16[this]==false) &&
- 	(value[this] == v) && (modulo(v,16) == 0); 
+procedure PackIntCellFew(divi: int, v:int, quot:int, this:Ref);
+requires (packedIntCellFew[this]==false);
+requires (value[this] == v);
+requires (divider[this] == divi);
+requires (quot <= 4);
 
-procedure UnpackMultipleOf16(v:int, this:Ref);
-requires packedMultipleOf16[this];
-requires fracMultipleOf16[this] > 0.0;
-ensures	(value[this] == v) && (modulo(v,16) == 0);
+procedure UnpackIntCellFew(divi: int, v:int, quot:int, this:Ref);
+requires packedIntCellFew[this];
+requires fracIntCellFew[this] > 0.0;
+ensures	(value[this] == v);
+ensures (divider[this] == divi);
+ensures (quot <= 4);
 
-procedure PackMultipleOf15(v:int, this:Ref);
-requires (packedMultipleOf15[this]==false) &&
- 	(value[this] == v) && (modulo(v,15) == 0); 
-
-procedure UnpackMultipleOf15(v:int, this:Ref);
-requires packedMultipleOf15[this];
-requires fracMultipleOf15[this] > 0.0;
-ensures	(value[this] == v) && (modulo(v,15) == 0);
-
-procedure PackMultipleOf14(v:int, this:Ref);
-requires (packedMultipleOf14[this]==false) &&
- 	(value[this] == v) && (modulo(v,14) == 0); 
-
-procedure UnpackMultipleOf14(v:int, this:Ref);
-requires packedMultipleOf14[this];
-requires fracMultipleOf14[this] > 0.0;
-ensures	(value[this] == v) && (modulo(v,14) == 0);
-
-procedure PackMultipleOf33(v:int, this:Ref);
-requires (packedMultipleOf33[this]==false) &&
- 	(value[this] == v) && (modulo(v,33) == 0); 
-
-procedure UnpackMultipleOf33(v:int, this:Ref);
-requires packedMultipleOf33[this];
-requires fracMultipleOf33[this] > 0.0;
-ensures	(value[this] == v) && (modulo(v,33) == 0);
-
-procedure PackMultipleOf4(v:int, this:Ref);
-requires (packedMultipleOf4[this]==false) &&
- 	(value[this] == v) && (modulo(v,4) == 0); 
-
-procedure UnpackMultipleOf4(v:int, this:Ref);
-requires packedMultipleOf4[this];
-requires fracMultipleOf4[this] > 0.0;
-ensures	(value[this] == v) && (modulo(v,4) == 0);
-
-procedure ConstructIntCell(x: int, this: Ref);
-	ensures (value[this] == x);
-
-procedure setValue(x: int, this: Ref) 
-modifies value;
+procedure ConstructIntCell(divider1: int, value1: int, this: Ref)
+modifies divider, value;
+ensures (value[this] == value1);
+ensures (divider[this] == divider1);
 {
-	value[this] := x;
+	value[this] := value1;
+	divider[this] := divider1;
 }
 
 procedure getValueInt(this: Ref) returns (r:int)
 {
-	r:=value[this];
+	r := value[this];
 }
 
