stateclient.bpl
@@ -1,3 +1,4 @@
+
 var scon: [Ref]Ref;
 
 var packedStateClientMultiple2:[Ref]bool;
@@ -6,71 +7,129 @@ var fracStateClientMultiple2:[Ref]real;
 var packedStateClientMultiple3:[Ref]bool;
 var fracStateClientMultiple3:[Ref]real;
 
-procedure PackStateClientMultiple2(s:Ref, this:Ref)
-requires (packedStateClientMultiple2[this] ==false);
+procedure PackStateClientMultiple2(s:Ref, this:Ref);
+requires (packedStateClientMultiple2[this] == false);
 requires (scon[this] == s);
 requires (fracStateContextMultiple2[s] > 0.0);
 
-procedure UnpackStateClientMultiple2(s:Ref, this:Ref)
+procedure UnpackStateClientMultiple2(s:Ref, this:Ref);
 requires packedStateClientMultiple2[this];
 requires fracStateClientMultiple2[this] > 0.0;
 ensures (scon[this] == s);
 ensures (fracStateContextMultiple2[s] > 0.0);
 
-procedure PackStateClientMultiple3(s:Ref, this:Ref)
-requires (packedStateClientMultiple3[this] ==false);
+procedure PackStateClientMultiple3(s:Ref, this:Ref);
+requires (packedStateClientMultiple3[this] == false);
 requires (scon[this] == s);
 requires (fracStateContextMultiple3[s] > 0.0);
 
-procedure UnpackStateClientMultiple3(s:Ref, this:Ref)
+procedure UnpackStateClientMultiple3(s:Ref, this:Ref);
 requires packedStateClientMultiple3[this];
 requires fracStateClientMultiple3[this] > 0.0;
 ensures (scon[this] == s);
 ensures (fracStateContextMultiple3[s] > 0.0);
 
-procedure stateClientCheckMultiplicity3(this:Ref) returns (r:bool)
-requires packedStateClientMultiple3[this];
-requires (fracStateClientMultiple3[this] >= 1.0);
-ensures packedStateClientMultiple3[this];
-ensures (fracStateClientMultiple3[this] >= 1.0);
+procedure ConstructStateClient(sco:Ref, this:Ref)
+modifies scon;
+ensures (scon[this] == sco);
 {
-call r:= stateContextCheckMultiplicity3(scon[this]);
+ scon[this] := sco; 
+}
+
+procedure stateClientCheckMultiplicity3(this:Ref) returns (r:bool)
+modifies packedStateContextMultiple3, packedStateClientMultiple3;
+requires packedStateClientMultiple3[this];
+requires (fracStateClientMultiple3[this] > 0.0);
+requires (forall  x:Ref :: ( packedStateClientMultiple3[x]));
+requires (forall  x:Ref :: ((instanceof[x] == 1)==> packedStateMultipleOf3StateLive[x])); 
+requires (forall  x:Ref :: ((instanceof[x] == 2)==> packedStateMultipleOf3StateLimbo[x])); 
+requires (forall  x:Ref :: ((instanceof[x] == 3)==> packedStateMultipleOf3StateSleep[x])); 
+requires (forall  x:Ref :: ( packedStateContextMultiple3[x])); 
+ensures packedStateClientMultiple3[this];
+ensures (fracStateClientMultiple3[this] > 0.0);
+ensures (forall  x:Ref :: ((instanceof[x] == 1)==> packedStateMultipleOf3StateLive[x])); 
+ensures (forall  x:Ref :: ((instanceof[x] == 2)==> packedStateMultipleOf3StateLimbo[x])); 
+ensures (forall  x:Ref :: ((instanceof[x] == 3)==> packedStateMultipleOf3StateSleep[x])); 
+ensures (forall  x:Ref :: ( packedStateContextMultiple3[x])); 
+ensures (forall  x:Ref :: ( packedStateClientMultiple3[x])); 
+{
+  call UnpackStateClientMultiple3(scon[this], this);
+  packedStateClientMultiple3[this] := false;
+  call r:= stateContextCheckMultiplicity3(scon[this]);
+  call PackStateClientMultiple3(scon[this], this);
+  packedStateClientMultiple3[this] := true;
 }
  
 procedure stateClientCheckMultiplicity2(this:Ref) returns (r:bool)
+modifies packedStateContextMultiple2, packedStateClientMultiple2;
 requires packedStateClientMultiple2[this];
-requires (fracStateClientMultiple2[this] >= 1.0);
+requires (fracStateClientMultiple2[this] > 0.0);
+requires (forall  x:Ref :: ( packedStateClientMultiple2[x]));
+requires (forall  x:Ref :: ((instanceof[x] == 1)==> packedStateMultipleOf2StateLive[x])); 
+requires (forall  x:Ref :: ((instanceof[x] == 2)==> packedStateMultipleOf2StateLimbo[x])); 
+requires (forall  x:Ref :: ((instanceof[x] == 3)==> packedStateMultipleOf2StateSleep[x])); 
+requires (forall  x:Ref :: ( packedStateContextMultiple2[x]));
 ensures packedStateClientMultiple2[this];
-ensures (fracStateClientMultiple2[this] >= 1.0);
+ensures (fracStateClientMultiple2[this] > 0.0);
+ensures (forall  x:Ref :: ((instanceof[x] == 1)==> packedStateMultipleOf2StateLive[x])); 
+ensures (forall  x:Ref :: ((instanceof[x] == 2)==> packedStateMultipleOf2StateLimbo[x])); 
+ensures (forall  x:Ref :: ((instanceof[x] == 3)==> packedStateMultipleOf2StateSleep[x])); 
+ensures (forall  x:Ref :: ( packedStateContextMultiple2[x])); 
+ensures (forall  x:Ref :: ( packedStateClientMultiple2[x]));
 {
-call r:= stateContextCheckMultiplicity2(scon[this]);
+  call UnpackStateClientMultiple2(scon[this], this);
+  packedStateClientMultiple2[this] := false;
+  call r := stateContextCheckMultiplicity2(scon[this]);
+  call PackStateClientMultiple2(scon[this], this);
+  packedStateClientMultiple2[this] := true;
 }
  
-procedure main(this:Ref)
+procedure main1(this:Ref)
+modifies cell, packedMultipleOf, fracMultipleOf, instanceof,
+        myState, divider, value, fracStateClientMultiple3,
+        packedStateClientMultiple3, packedStateMultipleOf3StateLive,
+        fracStateMultipleOf3StateLive, packedStateContextMultiple3,
+        fracStateContextMultiple3,   
+        packedStateLive, fracStateLive,
+        packedStateLimbo, fracStateLimbo, packedStateSleep, fracStateSleep,
+        packedStateMultipleOf3StateLimbo, 
+        packedStateMultipleOf3StateSleep, 
+        fracStateMultipleOf3StateLimbo, fracStateMultipleOf3StateSleep,
+        fracStateMultipleOf3StateLive, scon;
+requires (forall x:Ref :: ( packedMultipleOf[x]));
+requires (forall  x:Ref :: ( packedStateMultipleOf3StateLive[x])); 
+requires (forall  x:Ref :: ( packedStateMultipleOf3StateLimbo[x])); 
+requires (forall  x:Ref :: ( packedStateMultipleOf3StateSleep[x])); 
+requires (forall  x:Ref :: ( packedStateContextMultiple3[x])); 
+requires (forall  x:Ref :: ( packedStateClientMultiple3[x]));
 {
 var i1, i2 : Ref;
-var st1 : Ref;
-var scontext1 : Ref;
+var st1, st2 : Ref;
+var scontext1, scontext2 : Ref;
 var sclient1, sclient2, sclient3, sclient4 : Ref;
+var tempRef : Ref;
+var tempBool : bool;
 
-assume (i1!=i2);
+assume (i1 != i2);
+assume (st1 != st2);
 assume (sclient1 != sclient2);
 assume (sclient3 != sclient4);
+assume (scontext1 != scontext2);
 
-call ConstructIntCell(15, i1);
-packedMultipleOf15[i1] := false;
-call PackMultipleOf15(i1);
-packedMultipleOf15[i1] := true;
-fracMultipleOf15[i1] := 1.0;
+call ConstructIntCell(15, 15, i1);
+packedMultipleOf[i1] := false;
+call PackMultipleOf(15, 15, i1);
+packedMultipleOf[i1] := true;
+fracMultipleOf[i1] := 1.0;
+divider[i1]:=15;
 
-call ConstructStateLive(i1, st1);
+call ConstructStateLive2(i1, st1);
 packedStateMultipleOf3StateLive[st1] := false;
 call PackStateMultipleOf3StateLive(i1, st1);
 packedStateMultipleOf3StateLive[st1] := true;
 fracStateMultipleOf3StateLive[st1] := 1.0;
 
 instanceof[st1] := 1;
-
 call ConstructStateContext(st1, scontext1);
 packedStateContextMultiple3[scontext1] := false;
 call PackStateContextMultiple3(st1, scontext1);
@@ -89,20 +148,61 @@ call PackStateClientMultiple3(scontext1, sclient2);
 packedStateClientMultiple3[sclient2] := true;
 fracStateClientMultiple3[sclient2] := 1.0;
 
-call computeResult(1, scontext1);
-call stateClientCheckMultiplicity3(sclient1); 
-call computeResult(2, scontext1); 
-call stateClientCheckMultiplicity3(sclient2); 
-call computeResult(3, scontext1); 
-call stateClientCheckMultiplicity3(sclient1); 
+call UnpackStateContextMultiple3(myState[scontext1], scontext1);
+packedStateContextMultiple3[scontext1] := false;
+call tempRef := computeResultSC(1, scontext1);
+call tempBool := stateClientCheckMultiplicity3(sclient1); 
 
-call ConstructIntCell(14, i2);
-packedMultipleOf14[i2] := false;
-call PackMultipleOf14(i2);
-packedMultipleOf14[i2] := true;
-fracMultipleOf14[i2] := 1.0;
+call UnpackStateContextMultiple3(myState[scontext1], scontext1);
+packedStateContextMultiple3[scontext1] := false;
+call tempRef := computeResultSC(2, scontext1); 
+call tempBool := stateClientCheckMultiplicity3(sclient2); 
 
-call ConstructStateLive(i2, st2);
+call UnpackStateContextMultiple3(myState[scontext1], scontext1);
+packedStateContextMultiple3[scontext1] := false;
+call tempRef := computeResultSC(3, scontext1); 
+call tempBool := stateClientCheckMultiplicity3(sclient1); 		
+}
+
+procedure main2(this:Ref)
+modifies cell, packedMultipleOf, fracMultipleOf, instanceof,
+        myState, divider, value, 
+        packedStateMultipleOf2StateLive,
+        fracStateMultipleOf2StateLive, packedStateContextMultiple2,
+        fracStateContextMultiple2, packedStateClientMultiple2,
+        fracStateClientMultiple2, packedStateLive, fracStateLive,
+        packedStateLimbo, fracStateLimbo, packedStateSleep, fracStateSleep,
+        packedStateMultipleOf2StateLimbo,
+        packedStateMultipleOf2StateSleep,
+        fracStateMultipleOf2StateLimbo, fracStateMultipleOf2StateSleep, scon;
+requires (forall x:Ref :: ( packedMultipleOf[x]));
+requires (forall  x:Ref :: ( packedStateMultipleOf2StateLive[x])); 
+requires (forall  x:Ref :: ( packedStateMultipleOf2StateLimbo[x])); 
+requires (forall  x:Ref :: ( packedStateMultipleOf2StateSleep[x])); 
+requires (forall  x:Ref :: ( packedStateContextMultiple2[x])); 
+requires (forall  x:Ref :: ( packedStateClientMultiple2[x]));
+{
+var i1, i2 : Ref;
+var st1, st2 : Ref;
+var scontext1, scontext2 : Ref;
+var sclient1, sclient2, sclient3, sclient4 : Ref;
+var tempRef : Ref;
+var tempBool : bool;
+
+assume (i1 != i2);
+assume (st1 != st2);
+assume (sclient1 != sclient2);
+assume (sclient3 != sclient4);
+assume (scontext1 != scontext2);
+
+call ConstructIntCell(14, 14, i2);
+packedMultipleOf[i2] := false;
+call PackMultipleOf(14, 14, i2);
+packedMultipleOf[i2] := true;
+fracMultipleOf[i2] := 1.0;
+divider[i2] := 14;
+
+call ConstructStateLive2(i2, st2);
 packedStateMultipleOf2StateLive[st2] := false;
 call PackStateMultipleOf2StateLive(i2, st2);
 packedStateMultipleOf2StateLive[st2] := true;
@@ -128,11 +228,18 @@ call PackStateClientMultiple2(scontext2, sclient4);
 packedStateClientMultiple2[sclient4] := true;
 fracStateClientMultiple2[sclient4] := 1.0;
 
-call computeResult2(1, scontext2);
-call stateClientCheckMultiplicity2(sclient3); 
-call computeResult2(2, scontext2); 
-call stateClientCheckMultiplicity2(sclient4); 
-call computeResult2(3, scontext2); 
-call stateClientCheckMultiplicity2(sclient3); 			
+call UnpackStateContextMultiple2(myState[scontext2], scontext2);
+packedStateContextMultiple2[scontext2] := false;
+
+call tempRef := computeResult2SC(1, scontext2);
+call tempBool := stateClientCheckMultiplicity2(sclient3); 
+call UnpackStateContextMultiple2(myState[scontext2], scontext2);
+packedStateContextMultiple2[scontext2] := false;
+call tempRef := computeResult2SC(2, scontext2); 
+call tempBool := stateClientCheckMultiplicity2(sclient4); 
+call UnpackStateContextMultiple2(myState[scontext2], scontext2);
+packedStateContextMultiple2[scontext2] := false;
+call tempRef := computeResult2SC(3, scontext2); 
+call tempBool := stateClientCheckMultiplicity2(sclient3); 			
 }
 
