statecontext.bpl
@@ -1,7 +1,17 @@
+
 var myState: [Ref]Ref;
 
 var packedBasicFieldsContext : [Ref]bool;
 var fracBasicFieldsContext : [Ref]real;
+
+var packedStateLive :[Ref]bool;
+var fracStateLive :[Ref]real;
+
+var packedStateLimbo :[Ref]bool;
+var fracStateLimbo :[Ref]real;
+
+var packedStateSleep :[Ref]bool;
+var fracStateSleep :[Ref]real;
 
 var packedStateContextMultiple2 : [Ref]bool;
 var fracStateContextMultiple2 : [Ref]real;
@@ -12,53 +22,337 @@ var fracStateContextMultiple3 : [Ref]real;
 procedure PackStateContextMultiple2(m:Ref, this:Ref);
 requires (packedStateContextMultiple2[this] == false);
 requires (myState[this] == m);
-requires (instanceof[m] == 1) ==> (fracStateMultipleOf2StateLive[this] >= 1.0);
-requires (instanceof[m] == 2) ==> (fracStateMultipleOf2StateLimbo[this] >= 1.0);
-requires (instanceof[m] == 3) ==> (fracStateMultipleOf2StateSleep[this] >= 1.0);
+requires (instanceof[m] == 1) ==> (fracStateMultipleOf2StateLive[m] > 0.0);
+requires (instanceof[m] == 2) ==> (fracStateMultipleOf2StateLimbo[m] > 0.0);
+requires (instanceof[m] == 3) ==> (fracStateMultipleOf2StateSleep[m] > 0.0);
 
 procedure UnpackStateContextMultiple2(m:Ref, this:Ref);
 requires packedStateContextMultiple2[this];
 requires fracStateContextMultiple2[this] > 0.0;
 ensures (myState[this] == m);
-ensures (instanceof[m] == 1) ==> (fracStateMultipleOf2StateLive[this] >= 1.0);
-ensures (instanceof[m] == 2) ==> (fracStateMultipleOf2StateLimbo[this] >= 1.0);
-ensures (instanceof[m] == 3) ==> (fracStateMultipleOf2StateSleep[this] >= 1.0);
+ensures (instanceof[m] == 1) ==> (fracStateMultipleOf2StateLive[m] > 0.0);
+ensures (instanceof[m] == 2) ==> (fracStateMultipleOf2StateLimbo[m] > 0.0);
+ensures (instanceof[m] == 3) ==> (fracStateMultipleOf2StateSleep[m] > 0.0);
 
-//	predicate BasicFieldsContext() = exists m:StateLike :: this.myState -> m
+procedure PackStateContextMultiple3(m:Ref, this:Ref);
+requires (packedStateContextMultiple3[this] == false);
+requires (myState[this] == m);
+requires (instanceof[m] == 1) ==> (fracStateMultipleOf3StateLive[m] > 0.0);
+requires (instanceof[m] == 2) ==> (fracStateMultipleOf3StateLimbo[m] > 0.0);
+requires (instanceof[m] == 3) ==> (fracStateMultipleOf3StateSleep[m] > 0.0);
 
-//	predicate stateLive() = instanceof[myState]==1;
-//	predicate stateSleep() = instanceof[myState]==3;
-//	predicate stateLimbo() = instanceof[myState]==2;
-//	predicate stateContextMultiple2() = myState#1 StateMultipleOf2() 
-//	predicate stateContextMultiple3() = myState#1 StateMultipleOf3() 
+procedure UnpackStateContextMultiple3(m:Ref, this:Ref);
+requires packedStateContextMultiple3[this];
+requires fracStateContextMultiple3[this] > 0.0;
+ensures (myState[this] == m);
+ensures (instanceof[m] == 1) ==> (fracStateMultipleOf3StateLive[m] > 0.0);
+ensures (instanceof[m] == 2) ==> (fracStateMultipleOf3StateLimbo[m] > 0.0);
+ensures (instanceof[m] == 3) ==> (fracStateMultipleOf3StateSleep[m] > 0.0);
+
+procedure PackBasicFieldsContext(m:Ref, this:Ref);
+requires packedBasicFieldsContext[this] == false;
+requires (myState[this] == m);
+
+procedure UnpackBasicFieldsContext(m:Ref, this:Ref);
+requires packedBasicFieldsContext[this];
+requires fracBasicFieldsContext[this] > 0.0;
+ensures (myState[this] == m);
+
+procedure PackStateLive(m:Ref, this:Ref);
+requires packedStateLive[this] == false;
+requires fracStateLive[this] > 0.0;
+requires (myState[this] == m);
+requires instanceof[m]==1;
+
+procedure UnpackStateLive(m:Ref, this:Ref);
+requires packedStateLive[this];
+ensures (myState[this] == m);
+ensures instanceof[m]==1;
+
+procedure PackStateLimbo(m:Ref, this:Ref);
+requires packedStateLimbo[this] == false;
+requires fracStateLimbo[this] > 0.0;
+requires (myState[this] == m);
+requires instanceof[m]==2;
+
+procedure UnpackStateLimbo(m:Ref, this:Ref);
+requires  packedStateLimbo[this];
+ensures (myState[this] == m);
+ensures instanceof[m]==2;
+
+procedure PackStateSleep(m:Ref, this:Ref);
+requires packedStateSleep[this] == false;
+requires fracStateSleep[this] > 0.0;
+requires (myState[this] == m);
+requires instanceof[m]==3;
+
+procedure UnpackStateSleep(m:Ref, this:Ref);
+requires packedStateSleep[this];
+ensures (myState[this] == m);
+ensures instanceof[m]==3;
 	
-StateContext() 
-ensures this#1 stateLive() 
+procedure ConstructStateContext(mysta:Ref, this:Ref) 
+modifies myState;
+ensures myState[this] == mysta;
 { 
-	setState(new StateLive()); 
+  myState[this] := mysta;
+ // instanceof[myState[this]] := instanceof[mysta];
 } 
 
-void setState(Statelike newState) { 
-	myState = newState; 
+procedure setState2(newState:Ref, this:Ref) 
+modifies myState, instanceof, packedStateLive, fracStateLive
+       , packedStateLimbo, fracStateLimbo, packedStateSleep, fracStateSleep, 
+       packedStateContextMultiple2;
+requires (packedStateContextMultiple2[this] == false);
+requires (instanceof[newState] == 1) ==> (fracStateMultipleOf2StateLive[newState] > 0.0);
+requires (instanceof[newState] == 2) ==> (fracStateMultipleOf2StateLimbo[newState] > 0.0);
+requires (instanceof[newState] == 3) ==> (fracStateMultipleOf2StateSleep[newState] > 0.0);
+
+requires (forall  x:Ref :: ((instanceof[x]==1)==> packedStateMultipleOf2StateLive[x])); 
+requires (forall  x:Ref :: ((instanceof[x]==2)==>  packedStateMultipleOf2StateLimbo[x])); 
+requires (forall  x:Ref :: ((instanceof[x]==3)==>  packedStateMultipleOf2StateSleep[x])); 
+
+ensures myState[this] == newState;
+ensures instanceof[myState[this]] == instanceof[newState];
+
+ensures ((old(instanceof[newState]) == 1) ==> ( packedStateLive[this] && (fracStateLive[this] > 0.0)));
+ensures	((old(instanceof[newState]) == 2) ==> ( packedStateLimbo[this] && (fracStateLimbo[this] > 0.0)));
+ensures	((old(instanceof[newState]) == 3) ==> ( packedStateSleep[this] && (fracStateSleep[this] > 0.0)));
+ensures packedStateContextMultiple2[this];
+ensures (forall y:Ref :: (y!=myState[this]) ==> (instanceof[y] == old(instanceof[y]))); 
+ensures (forall y:Ref :: (y!=this) ==> (myState[y] == old(myState[y]))); 
+ensures (forall  x:Ref :: ((instanceof[x]==1)==> packedStateMultipleOf2StateLive[x])); 
+ensures (forall  x:Ref :: ((instanceof[x]==2)==>  packedStateMultipleOf2StateLimbo[x])); 
+ensures (forall  x:Ref :: ((instanceof[x]==3)==>  packedStateMultipleOf2StateSleep[x])); 
+ensures (forall  x:Ref :: ((x!=this) ==> (packedStateContextMultiple2[x] == old(packedStateContextMultiple2[x]))) ); 
+{ 
+	myState[this] := newState; 
+	instanceof[myState[this]] := instanceof[newState];
+  if (instanceof[newState] == 1 ) {
+     packedStateLive[this] := true;
+     fracStateLive[this] := 0.001;
+  } else
+  if (instanceof[newState] == 2 ) {
+     packedStateLimbo[this] := true;
+     fracStateLimbo[this] := 0.001;
+  } else
+  if (instanceof[newState] == 3 ) {
+     packedStateSleep[this] := true;
+     fracStateSleep[this] := 0.001;
+  } else {
+    assume false;
+  }
+
+  call PackStateContextMultiple2(myState[this], this);
+  packedStateContextMultiple2[this] := true;
 } 
 
-procedure computeResultSC(num: int) returns (r:Ref)
-modifies 
+
+procedure setState3(newState:Ref, this:Ref) 
+modifies myState, instanceof, packedStateLive, fracStateLive
+       , packedStateLimbo, fracStateLimbo, packedStateSleep, fracStateSleep, 
+       packedStateContextMultiple3;
+requires (packedStateContextMultiple3[this] == false);
+requires (instanceof[newState] == 1) ==> (fracStateMultipleOf3StateLive[newState] > 0.0);
+requires (instanceof[newState] == 2) ==> (fracStateMultipleOf3StateLimbo[newState] > 0.0);
+requires (instanceof[newState] == 3) ==> (fracStateMultipleOf3StateSleep[newState] > 0.0);
+requires (forall  x:Ref :: ((instanceof[x]==1)==> packedStateMultipleOf3StateLive[x])); 
+requires (forall  x:Ref :: ((instanceof[x]==2)==>  packedStateMultipleOf3StateLimbo[x])); 
+requires (forall  x:Ref :: ((instanceof[x]==3)==>  packedStateMultipleOf3StateSleep[x])); 
+ensures myState[this] == newState;
+ensures instanceof[myState[this]] == instanceof[newState];
+
+ensures ((old(instanceof[newState]) == 1) ==> ( packedStateLive[this] && (fracStateLive[this] > 0.0)));
+ensures	((old(instanceof[newState]) == 2) ==> ( packedStateLimbo[this] && (fracStateLimbo[this] > 0.0)));
+ensures	((old(instanceof[newState]) == 3) ==> ( packedStateSleep[this] && (fracStateSleep[this] > 0.0)));
 ensures packedStateContextMultiple3[this];
-ensures fracStateContextMultiple3[this] >= 1.0;
-ensures (old(instanceof[mystate[this]]) == 1) ==> (instanceof[mystate[this]] == 2);
-ensures (old(instanceof[mystate[this]]) == 2) ==> (instanceof[mystate[this]] == 3);
-ensures (old(instanceof[mystate[this]]) == 3) ==> (instanceof[mystate[this]] == 1);
+ensures (forall y:Ref :: (y!=myState[this]) ==> (instanceof[y] == old(instanceof[y]))); 
+ensures (forall y:Ref :: (y!=this) ==> (myState[y] == old(myState[y]))); 
+ensures (forall  x:Ref :: ((instanceof[x]==1)==> packedStateMultipleOf3StateLive[x])); 
+ensures (forall  x:Ref :: ((instanceof[x]==2)==>  packedStateMultipleOf3StateLimbo[x])); 
+ensures (forall  x:Ref :: ((instanceof[x]==3)==>  packedStateMultipleOf3StateSleep[x])); 
+ensures (forall  x:Ref :: ((x!=this) ==> (packedStateContextMultiple3[x] == old(packedStateContextMultiple3[x]))) ); 
+{ 
+	myState[this] := newState; 
+	instanceof[myState[this]] := instanceof[newState];
+  if (instanceof[newState] == 1 ) {
+     packedStateLive[this] := true;
+     fracStateLive[this] := 0.001;
+  } else
+  if (instanceof[newState] == 2 ) {
+     packedStateLimbo[this] := true;
+     fracStateLimbo[this] := 0.001;
+  } else
+  if (instanceof[newState] == 3 ) {
+     packedStateSleep[this] := true;
+     fracStateSleep[this] := 0.001;
+  } else {
+    assume false;
+  }
+  call PackStateContextMultiple3(myState[this], this);
+  packedStateContextMultiple3[this] := true;
+     
+} 
+
+procedure computeResultSC(num: int, this:Ref) returns (r:Ref)
+modifies cell, value, myState, instanceof, packedStateLive, fracStateLive,
+        packedStateMultipleOf3StateLive , packedStateLimbo, fracStateLimbo
+        , packedStateSleep, fracStateSleep, divider, packedMultipleOf, fracMultipleOf,
+        packedStateContextMultiple3, packedStateMultipleOf3StateLimbo, 
+        packedStateMultipleOf3StateSleep, fracStateMultipleOf3StateLimbo,
+        fracStateMultipleOf3StateSleep, fracStateMultipleOf3StateLive;
+requires packedStateContextMultiple3[this]==false;
+requires fracStateContextMultiple3[this] > 0.0;
+requires (instanceof[myState[this]] == 1) ==> (
+      packedStateMultipleOf3StateLive[myState[this]] &&
+      (fracStateMultipleOf3StateLive[myState[this]] > 0.0)
+);
+requires (instanceof[myState[this]] == 2) ==> (
+      packedStateMultipleOf3StateLimbo[myState[this]] &&
+      (fracStateMultipleOf3StateLimbo[myState[this]] > 0.0)
+);
+requires (instanceof[myState[this]] == 3) ==> (
+      packedStateMultipleOf3StateSleep[myState[this]] &&
+      (fracStateMultipleOf3StateSleep[myState[this]] > 0.0)
+);
+requires (forall  x:Ref :: ((instanceof[x]==1)==> packedStateMultipleOf3StateLive[x])); 
+requires (forall  x:Ref :: ((instanceof[x]==2)==>  packedStateMultipleOf3StateLimbo[x])); 
+requires (forall  x:Ref :: ((instanceof[x]==3)==>  packedStateMultipleOf3StateSleep[x])); 
+requires (forall  x:Ref :: ((x!=this) ==> packedStateContextMultiple3[x])); 
+//requires (forall x:Ref :: ( packedMultipleOf[x]));
+ensures packedStateContextMultiple3[this];
+ensures fracStateContextMultiple3[this] > 0.0;
+ensures (forall  x:Ref :: ((instanceof[x]==1)==> packedStateMultipleOf3StateLive[x])); 
+ensures (forall  x:Ref :: ((instanceof[x]==2)==>  packedStateMultipleOf3StateLimbo[x])); 
+ensures (forall  x:Ref :: ((instanceof[x]==3)==>  packedStateMultipleOf3StateSleep[x])); 
+ensures (forall  x:Ref :: ( packedStateContextMultiple3[x])); 
+//ensures (forall x:Ref :: ( packedMultipleOf[x]));
 {
-var temp : Ref;
-if (instanceof[myState[this]]) == 1) {
-	call temp := computeResultStateLive(this, num, myState[this]);
-} else if (instanceof[mystate[this]]) == 2) {
-	call temp := computeResultStateLimbo(this, num, myState[this]);
+if (instanceof[myState[this]] == 1) {
+	call r := computeResultStateLive(this, num, myState[this]);
+} else if (instanceof[myState[this]] == 2)  {
+	call r := computeResultStateLimbo(this, num, myState[this]);
+} else if (instanceof[myState[this]] == 3)  {
+	call r := computeResultStateSleep(this, num, myState[this]);
+} 
+else {
+  // We cannot be in this else and we 
+  // express this like below.
+  assume false;
+}
+}
+
+procedure computeResult2SC(num: int, this:Ref) returns (r:Ref)
+modifies cell, value, myState, instanceof, packedStateLive, fracStateLive
+         , packedStateLimbo, fracStateLimbo, packedStateSleep, fracStateSleep
+         , packedStateContextMultiple2, divider, packedMultipleOf, fracMultipleOf,
+         packedStateMultipleOf2StateLimbo, fracStateMultipleOf2StateLimbo,
+         packedStateMultipleOf2StateSleep, fracStateMultipleOf2StateSleep,
+          packedStateMultipleOf2StateLive, fracStateMultipleOf2StateLive;
+requires packedStateContextMultiple2[this]==false;
+requires fracStateContextMultiple2[this] > 0.0;
+requires (instanceof[myState[this]] == 1) ==> (
+      packedStateMultipleOf2StateLive[myState[this]] &&
+      (fracStateMultipleOf2StateLive[myState[this]] > 0.0)
+);
+requires (instanceof[myState[this]] == 2) ==> (
+      packedStateMultipleOf2StateLimbo[myState[this]] &&
+      (fracStateMultipleOf2StateLimbo[myState[this]] > 0.0)
+);
+requires (instanceof[myState[this]] == 3) ==> (
+      packedStateMultipleOf2StateSleep[myState[this]] &&
+      (fracStateMultipleOf2StateSleep[myState[this]] > 0.0)
+);
+//requires (forall x:Ref :: ( packedMultipleOf[x]));
+requires (forall  x:Ref :: ((instanceof[x]==1)==> packedStateMultipleOf2StateLive[x])); 
+requires (forall  x:Ref :: ((instanceof[x]==2)==>  packedStateMultipleOf2StateLimbo[x])); 
+requires (forall  x:Ref :: ((instanceof[x]==3)==>  packedStateMultipleOf2StateSleep[x])); 
+requires (forall  x:Ref :: ((x!=this) ==> packedStateContextMultiple2[x])); 
+ensures packedStateContextMultiple2[this];
+ensures fracStateContextMultiple2[this] > 0.0;
+
+ensures (forall  x:Ref :: ((instanceof[x]==1)==> packedStateMultipleOf2StateLive[x])); 
+ensures (forall  x:Ref :: ((instanceof[x]==2)==> packedStateMultipleOf2StateLimbo[x])); 
+ensures (forall  x:Ref :: ((instanceof[x]==3)==> packedStateMultipleOf2StateSleep[x])); 
+ensures (forall  x:Ref :: ( packedStateContextMultiple2[x])); 
+//ensures (forall x:Ref :: ( packedMultipleOf[x]));
+{
+if (instanceof[myState[this]] == 1) {
+	call r := computeResult2StateLive(this, num, myState[this]);
+} else if (instanceof[myState[this]] == 2) {
+	call r := computeResult2StateLimbo(this, num, myState[this]);
+} else if (instanceof[myState[this]] == 3) {
+	call r := computeResult2StateSleep(this, num, myState[this]);
 } else {
-	call temp := computeResultStateSleep(this, num, myState[this]);
+  assume false;
+}
 }
 
+procedure stateContextCheckMultiplicity3(this:Ref) returns (b:bool) 
+modifies packedStateContextMultiple3;
+requires packedStateContextMultiple3[this];
+requires fracStateContextMultiple3[this] > 0.0;
+requires (forall  x:Ref :: ( packedStateContextMultiple3[x])); 
+requires (forall  x:Ref :: ((instanceof[x] == 1)==> packedStateMultipleOf3StateLive[x])); 
+requires (forall  x:Ref :: ((instanceof[x] == 2)==> packedStateMultipleOf3StateLimbo[x])); 
+requires (forall  x:Ref :: ((instanceof[x] == 3)==> packedStateMultipleOf3StateSleep[x])); 
+ensures packedStateContextMultiple3[this];
+ensures fracStateContextMultiple3[this] > 0.0; 
+ensures (forall  x:Ref :: ( packedStateContextMultiple3[x])); 
+{ 
+   call UnpackStateContextMultiple3(myState[this], this);
+  packedStateContextMultiple3[this] := false;
+if (instanceof[myState[this]] == 1) {
+	call b := checkMod3StateLive(myState[this]);
+  call PackStateContextMultiple3(myState[this], this);
+  packedStateContextMultiple3[this] := true;
+} else if (instanceof[myState[this]] == 2) {
+	call b := checkMod3StateLimbo(myState[this]);
+  call PackStateContextMultiple3(myState[this], this);
+  packedStateContextMultiple3[this] := true;
+} else if (instanceof[myState[this]] == 3){
+	call b := checkMod3StateSleep(myState[this]);
+  call PackStateContextMultiple3(myState[this], this);
+  packedStateContextMultiple3[this] := true;
+} else {
+  // This means we cannot end up in this else.
+  assume false;
 }
+} 
 
+procedure stateContextCheckMultiplicity2(this:Ref) returns (b:bool) 
+modifies packedStateContextMultiple2;
+requires packedStateContextMultiple2[this];
+requires fracStateContextMultiple2[this] > 0.0;
+requires (forall  x:Ref :: ( packedStateContextMultiple2[x])); 
+requires (forall  x:Ref :: ((instanceof[x] == 1)==> packedStateMultipleOf2StateLive[x])); 
+requires (forall  x:Ref :: ((instanceof[x] == 2)==> packedStateMultipleOf2StateLimbo[x])); 
+requires (forall  x:Ref :: ((instanceof[x] == 3)==> packedStateMultipleOf2StateSleep[x])); 
+ensures packedStateContextMultiple2[this];
+ensures fracStateContextMultiple2[this] > 0.0;
+ensures (forall  x:Ref :: ( packedStateContextMultiple2[x])); 
+{ 
+if (instanceof[myState[this]] == 1) {
+  call UnpackStateContextMultiple2(myState[this], this);
+  packedStateContextMultiple2[this] := false;
+	call b := checkMod2StateLive(myState[this]);
+  call PackStateContextMultiple2(myState[this], this);
+  packedStateContextMultiple2[this] := true;
+} else if (instanceof[myState[this]] == 2) {
+  call UnpackStateContextMultiple2(myState[this], this);
+  packedStateContextMultiple2[this] := false;
+	call b := checkMod2StateLimbo(myState[this]);
+  call PackStateContextMultiple2(myState[this], this);
+  packedStateContextMultiple2[this] := true;
+} else if (instanceof[myState[this]] == 3) {
+  call UnpackStateContextMultiple2(myState[this], this);
+  packedStateContextMultiple2[this] := false;
+	call b := checkMod2StateSleep(myState[this]);
+  call PackStateContextMultiple2(myState[this], this);
+  packedStateContextMultiple2[this] := true;
+} else {
+  // This means we cannot end up in this else.
+  assume false;
+}
+} 
 
