statelive.bpl
@@ -1,12 +1,6 @@
-type Ref;
-
-const null: Ref;
 
 var cell : [Ref]Ref;
 var instanceof : [Ref]int;
-
-var packedBasicFieldsStateLive: [Ref] bool;
-var fracBasicFieldsStateLive: [Ref] real;
 
 var packedStateMultipleOf3StateLive: [Ref]bool;
 var fracStateMultipleOf3StateLive: [Ref]real;
@@ -14,95 +8,148 @@ var fracStateMultipleOf3StateLive: [Ref]real;
 var packedStateMultipleOf2StateLive: [Ref]bool;
 var fracStateMultipleOf2StateLive: [Ref]real;
 
-procedure PackBasicFieldsStateLive(c: Ref, this: Ref)
-requires (packedBasicFieldsStateLive[this] == false);
+procedure PackStateMultipleOf3StateLive(c:Ref, this:Ref);
+requires (packedStateMultipleOf3StateLive[this] == false);
 requires (cell[this] == c);
+requires (fracMultipleOf[c] > 0.0);
+requires (divider[cell[this]] == 15);
 
-procedure UnpackBasicFieldsStateLive(c: Ref, this: Ref)
-requires packedBasicFieldsStateLive[this];
-requires fracBasicFieldsStateLive[this] > 0.0;
-ensures (cell[this] == c);
-
-procedure PackStateMultipleOf3StateLive(c:Ref, this:Ref)
-requires (packedStateMultipleOf3StateLive[this] ==false);
-requires (cell[this] == c);
-requires (fracMultipleOf15[c] == 1.0);
-
-procedure UnpackStateMultipleOf3StateLive(c:Ref, this:Ref)
+procedure UnpackStateMultipleOf3StateLive(c:Ref, this:Ref);
 requires packedStateMultipleOf3StateLive[this];
 requires fracStateMultipleOf3StateLive[this] > 0.0;
 ensures (cell[this] == c);
-ensures (fracMultipleOf15[c] == 1.0);
+ensures (fracMultipleOf[c] > 0.0);
+ensures (divider[cell[this]] == 15);
 
-procedure PackStateMultipleOf2StateLive(c:Ref, this:Ref)
+procedure PackStateMultipleOf2StateLive(c:Ref, this:Ref);
 requires (packedStateMultipleOf2StateLive[this] ==false);
 requires (cell[this] == c);
-requires (fracMultipleOf14[c] == 1.0);
+requires (fracMultipleOf[c] > 0.0);
+requires (divider[cell[this]] == 14);
 
-procedure UnpackStateMultipleOf2StateLive(c:Ref, this:Ref)
+procedure UnpackStateMultipleOf2StateLive(c:Ref, this:Ref);
 requires packedStateMultipleOf2StateLive[this];
 requires fracStateMultipleOf2StateLive[this] > 0.0;
 ensures (cell[this] == c);
-ensures (fracMultipleOf14[c] == 1.0);
+ensures (fracMultipleOf[c] > 0.0);
+ensures (divider[cell[this]] == 14);
 
-procedure ConstructStateLive(this:Ref);
+procedure ConstructStateLive(this:Ref)
+modifies cell, divider, value;
+//ensures (forall y:Ref :: ( (y!=this) ==> (cell[y] == old(cell[y]) ) ) );
 {	
 	var temp:Ref;
-	call ConstructIntCell(0, temp);
-	call ConstructStateLive(temp, cell[this]);
+	call ConstructIntCell(1, 0, temp);
+	call ConstructStateLive2(temp, cell[this]);
 }
 
-procedure ConstructStateLive(c:Ref, this:Ref);
+procedure ConstructStateLive2(c:Ref, this:Ref)
+modifies cell;
 ensures cell[this] == c;
 {	
 	cell[this] := c;
 }
 
-procedure computeResultStateLive(context:Ref, num:int) returns (r:Ref)
-modifies cell;
-requires packedBasicFieldsStateLive[this] && (fracBasicFieldsStateLive[this] >= 1.0);
-requires packedBasicFieldsContext[context] && (fracBasicFieldsContext[context] >= 1.0);
-ensures packedStateMultipleOf3StateLive[this] && (fracStateMultipleOf3StateLive[this] >= 1.0);
-ensures packedStateLimbo[context] && (fracStateLimbo[context] >= 1.0)
+procedure computeResultStateLive(context:Ref, num:int, this:Ref) returns (r:Ref)
+modifies cell, value, myState, instanceof, packedStateLive, fracStateLive, 
+         packedStateLimbo, fracStateLimbo, packedStateSleep, fracStateSleep, packedStateMultipleOf3StateLimbo
+         , fracStateMultipleOf3StateLimbo, divider, packedMultipleOf, fracMultipleOf,
+         packedStateContextMultiple3;
+requires (packedStateContextMultiple3[context]==false);
+requires (fracStateContextMultiple3[context] > 0.0);
+requires (forall  x:Ref :: ((instanceof[x]==1)==> packedStateMultipleOf3StateLive[x])); 
+requires (forall  x:Ref :: ((instanceof[x]==2)==>  packedStateMultipleOf3StateLimbo[x])); 
+requires (forall  x:Ref :: ((instanceof[x]==3)==>  packedStateMultipleOf3StateSleep[x])); 
+ensures (packedStateContextMultiple3[context]==true);
+ensures (fracStateContextMultiple3[context] > 0.0);
+ensures packedStateLimbo[context];
+ensures	(fracStateLimbo[context] > 0.0);
+ensures (forall  x:Ref :: ((instanceof[x]==1)==> packedStateMultipleOf3StateLive[x])); 
+ensures (forall  x:Ref :: ((instanceof[x]==2)==>  packedStateMultipleOf3StateLimbo[x])); 
+ensures (forall  x:Ref :: ((instanceof[x]==3)==>  packedStateMultipleOf3StateSleep[x])); 
+ensures (forall  x:Ref :: ((x!=context) ==> (packedStateContextMultiple3[x] == old(packedStateContextMultiple3[x]))) ); 
 {
-var s : Ref;
-call ConstructStateLimbo(s);
-// StateLike s = new StateLimbo()[];
-call setValue(num*15, cell[this]);
-call setState(s, context);
-r:=cell[this];
+var i1:Ref;
+assume (r!=this);
+
+call ConstructIntCell(21, num*21, i1);
+packedMultipleOf[i1] := false;
+call PackMultipleOf(21, num*21, i1);
+packedMultipleOf[i1] := true;
+fracMultipleOf[i1] := 1.0;
+divider[i1]:=21;
+
+call ConstructStateLimbo2(i1, r);
+packedStateMultipleOf3StateLimbo[r] := false;
+call PackStateMultipleOf3StateLimbo(i1, r);
+packedStateMultipleOf3StateLimbo[r] := true;
+fracStateMultipleOf3StateLimbo[r] := 1.0;
+
+instanceof[r] := 2;
+call setState3(r, context);
 }
 
-procedure computeResult2StateLive(context:Ref, num:int) returns (r:Ref)
-modifies cell;
-requires packedBasicFieldsStateLive[this] && (fracBasicFieldsStateLive[this] >= 1.0);
-requires packedBasicFieldsContext[context] && (fracBasicFieldsContext[context] >= 1.0);
-ensures packedStateMultipleOf2StateLive[this] && (fracStateMultipleOf2StateLive[this] >= 1.0);
-ensures packedStateSleep[context] && (fracStateSleep[context] >= 1.0)
+procedure computeResult2StateLive(context:Ref, num:int, this:Ref) returns (r:Ref)
+modifies cell, value, myState, instanceof, packedStateLive, fracStateLive
+         , packedStateLimbo, fracStateLimbo, packedStateSleep, fracStateSleep
+         , divider, packedMultipleOf, fracMultipleOf, packedStateMultipleOf2StateLive,
+         fracStateMultipleOf2StateSleep, packedStateMultipleOf2StateSleep,
+         packedStateContextMultiple2;
+requires (packedStateContextMultiple2[context] == false);
+requires (fracStateContextMultiple2[context] > 0.0);
+requires (forall  x:Ref :: ((instanceof[x]==1)==> packedStateMultipleOf2StateLive[x])); 
+requires (forall  x:Ref :: ((instanceof[x]==2)==>  packedStateMultipleOf2StateLimbo[x])); 
+requires (forall  x:Ref :: ((instanceof[x]==3)==>  packedStateMultipleOf2StateSleep[x])); 
+ensures (packedStateContextMultiple2[context] == true);
+ensures (fracStateContextMultiple2[context] > 0.0);
+ensures packedStateSleep[context];
+ensures	(fracStateSleep[context] > 0.0);
+ensures (forall  x:Ref :: ((instanceof[x]==1)==> packedStateMultipleOf2StateLive[x])); 
+ensures (forall  x:Ref :: ((instanceof[x]==2)==>  packedStateMultipleOf2StateLimbo[x])); 
+ensures (forall  x:Ref :: ((instanceof[x]==3)==>  packedStateMultipleOf2StateSleep[x])); 
+ensures (forall  x:Ref :: ((x!=context) ==> (packedStateContextMultiple2[x] == old(packedStateContextMultiple2[x]))) ); 
 {
-var s : Ref;
-call ConstructStateSleep(s);
+var i1:Ref;
+assume (r!=this);
+
+call ConstructIntCell(4, num*4, i1);
+packedMultipleOf[i1] := false;
+call PackMultipleOf(4, num*4, i1);
+packedMultipleOf[i1] := true;
+fracMultipleOf[i1] := 1.0;
+divider[i1]:=4;
+
+call ConstructStateSleep2(i1, r);
+packedStateMultipleOf2StateSleep[r] := false;
+call PackStateMultipleOf2StateSleep(i1, r);
+packedStateMultipleOf2StateSleep[r] := true;
+fracStateMultipleOf2StateSleep[r] := 1.0;
+
+instanceof[r] := 3;
+
 // StateLike s = new StateSleep()[];
-call setValue(num*14, cell[this]);
-call setState(s, context);
-r:=cell[this];
+call setState2(r, context);
 }
 
 procedure checkMod3StateLive(this:Ref) returns (b:bool)
-requires packedStateMultipleOf3StateLive[this] && (fracStateMultipleOf3StateLive[this] >= 1.0);
-ensures packedStateMultipleOf3StateLive[this] && (fracStateMultipleOf3StateLive[this] >= 1.0);
+requires packedStateMultipleOf3StateLive[this];
+requires (fracStateMultipleOf3StateLive[this] > 0.0);
+ensures packedStateMultipleOf3StateLive[this];
+requires (fracStateMultipleOf3StateLive[this] > 0.0);
 {
 var temp : int;
-call temp :=getValueInt(cell[this]);
-r:= (modulo(temp, 3) == 0);
+call temp := getValueInt(cell[this]);
+b:= (modulo(temp, 3) == 0);
 }
 
 procedure checkMod2StateLive(this:Ref) returns (b:bool)
-requires packedStateMultipleOf2StateLive[this] && (fracStateMultipleOf2StateLive[this] >= 1.0);
-ensures packedStateMultipleOf2StateLive[this] && (fracStateMultipleOf2StateLive[this] >= 1.0);
+requires packedStateMultipleOf2StateLive[this];
+requires (fracStateMultipleOf2StateLive[this] > 0.0);
+ensures packedStateMultipleOf2StateLive[this];
+requires (fracStateMultipleOf2StateLive[this] > 0.0);
 {
 var temp : int;
 call temp :=getValueInt(cell[this]);
-r:= (modulo(temp, 2) == 0);
+b:= (modulo(temp, 2) == 0);
 }
 
