studentapplication.bpl
@@ -1,6 +1,8 @@
+
 var college : [Ref]Ref;
 var campusNumber : [Ref]int;
-var facilities : [Ref]Ref;
+// facilities is a field of StudentApplication
+var facilities : [Ref]int;
 
 var packedStudentApplicationFields : [Ref]bool;
 var fracStudentApplicationFields : [Ref]real;
@@ -13,93 +15,134 @@ var fracStudentAppFacilitiesFew : [Ref]real;
 
 procedure PackStudentApplicationFields(c:Ref, camp:int, this:Ref);
 requires packedStudentApplicationFields[this] == false;
-requires (college[this] == c) && (campusNumber[this] == camp);
+requires (college[this] == c);
+requires (campusNumber[this] == camp);
 
 procedure UnpackStudentApplicationFields(c:Ref, camp:int, this:Ref);
 requires packedStudentApplicationFields[this];
-ensures (college[this] == c) && (campusNumber[this] == camp);
+ensures (college[this] == c);
+ensures	(campusNumber[this] == camp);
 
-procedure PackStudentAppFacilitiesMany(col:Ref, c:int, f:Ref, this:Ref);
+procedure PackStudentAppFacilitiesMany(col:Ref, c:int, this:Ref);
 requires packedStudentAppFacilitiesMany[this] == false;
-requires (college[this] == col) && (campusNumber[this] == c) &&
-	(facilities[this] == f) && 
-	packedCollegeFacilitiesMany[col] &&
-	(fracCollegeFacilitiesMany[col] > 0.0);
+requires (college[this] == col);
+requires (campusNumber[this] == c);
+requires packedCollegeFacilitiesMany[col];
+requires (fracCollegeFacilitiesMany[col] > 0.0);
 //TODO add ensures about params in this object proposition
 
 procedure UnpackStudentAppFacilitiesMany(col:Ref, c:int, this:Ref);
 requires packedStudentAppFacilitiesMany[this];
 requires fracStudentAppFacilitiesMany[this] > 0.0;
-ensures (college[this] == col) && (campusNumber[this] == c) &&
-	packedCollegeFacilitiesMany[col] &&
-	(fracCollegeFacilitiesMany[col] > 0.0);
+ensures (college[this] == col);
+ensures	(campusNumber[this] == c);
+ensures	packedCollegeFacilitiesMany[col];
+ensures	(fracCollegeFacilitiesMany[col] > 0.0);
 
 procedure PackStudentAppFacilitiesFew(col:Ref, c:int, this:Ref);
 requires packedStudentAppFacilitiesFew[this] == false;
-requires (college[this] == col) && (campusNumber[this] == c) &&
-	packedCollegeFacilitiesFew[col] &&
-	(fracCollegeFacilitiesFew[col] > 0.0);
+requires (college[this] == col);
+requires (campusNumber[this] == c);
+requires packedCollegeFacilitiesFew[col];
+requires (fracCollegeFacilitiesFew[col] > 0.0);
 //TODO add ensures about params in this object proposition
 
 procedure UnpackStudentAppFacilitiesFew(col:Ref, c:int, this:Ref);
 requires packedStudentAppFacilitiesFew[this];
 requires fracStudentAppFacilitiesFew[this] > 0.0;
-ensures (college[this] == col) && (campusNumber[this] == c) &&
-	packedCollegeFacilitiesFew[col] &&
-	(fracCollegeFacilitiesFew[col] > 0.0);
+ensures (college[this] == col);
+ensures	(campusNumber[this] == c);
+ensures	packedCollegeFacilitiesFew[col];
+ensures	(fracCollegeFacilitiesFew[col] > 0.0);
 
 procedure ConstructStudentApplication(col:Ref, campusNum:int, this:Ref) 
-modifies college, facilities, campusNumber;
-ensures packedStudentApplicationFields[this] &&
-	(fracStudentApplicationFields[this] == 1.0)
+modifies college, facilities, campusNumber, fracMultipleOf, packedMultipleOf, divider, value,
+        packedCollegeFacilitiesFew, packedCollegeFacilitiesMany
+        , fracCollegeFacilitiesFew, fracCollegeFacilitiesMany;
+  requires campusNum > 0;
+  ensures (college[this] == col);
+  ensures (campusNumber[this] == campusNum);
+  ensures ( (campusNum <= 4) && (campusNum > 0)  )==> ( packedCollegeFacilitiesFew[col] && 
+	(fracCollegeFacilitiesFew[col] > 0.0) );
+  ensures (campusNum >= 10) ==> ( packedCollegeFacilitiesMany[col] &&
+	(fracCollegeFacilitiesMany[col] > 0.0) );
 {
+    var temp : int;
+    assume (forall y:Ref :: (collegeNumber[y] > 0) );
 		college[this] := col;
-		call facilities[this] := getNumberFacilities(campusNum, college[this]);
+		call temp := getNumberFacilities(campusNum, collegeNumber[college[this]], college[this]);
+    facilities[this] := temp;// !!!Here I need to add in the Java program what is the
+    // new predicate that has to hold about col, because only now I have all the information
+    // to know which predicate holds.
+    // I have a fraction to col since it is given as input.
 		campusNumber[this] := campusNum;	
+    if (0 < campusNum  && campusNum <= 4) {
+      packedCollegeFacilitiesFew[college[this]] := false;
+      call PackCollegeFacilitiesFew(facilities[this], collegeNumber[college[this]], college[this]);
+      packedCollegeFacilitiesFew[college[this]] := true;
+      fracCollegeFacilitiesFew[college[this]] := 0.001;
+      
+    } else if (campusNum >= 10) {
+      packedCollegeFacilitiesMany[college[this]] := false;
+      call PackCollegeFacilitiesMany(facilities[this] ,collegeNumber[college[this]], college[this]);
+      packedCollegeFacilitiesMany[college[this]] := true;
+      fracCollegeFacilitiesMany[college[this]] := 0.001;
+    }
 }
-	
+
 procedure changeApplicationFew(newCampusNumber:int, this:Ref)
-modifies campusNumber, facilities;
-requires packedStudentAppFacilitiesFew[this] &&
-	(fracStudentAppFacilitiesFew[this] == 1.0);
-ensures packedStudentAppFacilitiesFew[this] &&
-	(fracStudentAppFacilitiesFew[this] == 1.0);
+modifies campusNumber, facilities, fracMultipleOf, packedMultipleOf, divider, value,
+        packedStudentAppFacilitiesFew, packedStudentAppFacilitiesMany;
+requires newCampusNumber > 0;
+requires packedStudentAppFacilitiesFew[this];
+requires (fracStudentAppFacilitiesFew[this] > 0.0);
+ensures packedStudentAppFacilitiesFew[this];
+ensures	(fracStudentAppFacilitiesFew[this] > 0.0);
+ensures (forall y:Ref :: ( (y!=this) ==> (packedStudentAppFacilitiesFew[y] == old(packedStudentAppFacilitiesFew[y]) ) ) );
 {
-	campusNumber[this] := modulo(newCampusNumber, 4);
-	call facilities[this] := getNumberFacilities(campusNumber[this], college[this]);
+  var temp : int;
+  assume (forall y:Ref :: (collegeNumber[y] > 0) );
+	campusNumber[this] := modulo(newCampusNumber, 4) + 1;
+  call UnpackStudentAppFacilitiesFew(college[this], campusNumber[this], this);
+  packedStudentAppFacilitiesFew[this] := false;
+	call temp := getNumberFacilities(campusNumber[this], collegeNumber[college[this]], college[this]);
+  facilities[this] := temp;
+  call PackStudentAppFacilitiesFew(college[this], campusNumber[this], this);
+  packedStudentAppFacilitiesFew[this] := true;
 }
 
 procedure changeApplicationMany(newCampusNumber:int, this:Ref)
-modifies campusNumber, facilities;
-requires packedStudentAppFacilitiesMany[this] &&
-	(fracStudentAppFacilitiesMany[this] == 1.0);
-ensures packedStudentAppFacilitiesMany[this] &&
-	(fracStudentAppFacilitiesMany[this] == 1.0);
+modifies campusNumber, facilities, fracMultipleOf, packedMultipleOf, divider, value;
+requires newCampusNumber > 0;
+requires packedStudentAppFacilitiesMany[this];
+requires (fracStudentAppFacilitiesMany[this] > 0.0);
+ensures packedStudentAppFacilitiesMany[this];
+ensures	(fracStudentAppFacilitiesMany[this] > 0.0);
 {
-	campusNumber[this] := newCampusNumber * 10 + 1;
-	call facilities[this] := getNumberFacilities(campusNumber[this], college[this]);
+  	var temp:int; 
+    assume (forall y:Ref :: (collegeNumber[y] > 0) );
+	  campusNumber[this] := newCampusNumber * 10 + 1;
+	  call temp := getNumberFacilities(campusNumber[this],collegeNumber[college[this]], college[this]);
+  	facilities[this] := temp;
 }
 
 
 procedure checkFacilitiesFew(this:Ref) returns (b:bool)
-requires packedStudentAppFacilitiesFew[this] &&
-	(fracStudentAppFacilitiesFew[this] == 1.0);
-ensures packedStudentAppFacilitiesFew[this] &&
-	(fracStudentAppFacilitiesFew[this] == 1.0);
+requires packedStudentAppFacilitiesFew[this];
+requires (fracStudentAppFacilitiesFew[this] > 0.0);
+ensures packedStudentAppFacilitiesFew[this];
+ensures	(fracStudentAppFacilitiesFew[this] > 0.0);
 {        
-	var temp:bool;
-	call temp := getValueInt(facilities[this]);
-	b := (temp <= 4 * campusNumber[this]);
+	b := (facilities[this] <= 4 * campusNumber[this]);
 }
 
 procedure checkFacilitiesMany(this:Ref) returns (b:bool)
-requires packedStudentAppFacilitiesMany[this] &&
-	(fracStudentAppFacilitiesMany[this] == 1.0);
-ensures packedStudentAppFacilitiesMany[this] &&
-	(fracStudentAppFacilitiesMany[this] == 1.0);
+requires packedStudentAppFacilitiesMany[this];
+requires (fracStudentAppFacilitiesMany[this] > 0.0);
+ensures packedStudentAppFacilitiesMany[this];
+ensures	(fracStudentAppFacilitiesMany[this] > 0.0);
 {       
-	var temp:bool;
-	call temp := getValueInt(facilities[this]);
-	b := (temp >= 10 * campusNumber[this]);
+	b := (facilities[this] >= 10 * campusNumber[this]);
 }
+
 
