clientsum.bpl
@@ -1,3 +1,4 @@
+
 var sumClient : [Ref]Ref;
 var instanceof: [Ref]int; // maybe this should be declared in the interface Sum
 // actually it's ok to be declared in the first class that implements the interface because
@@ -8,58 +9,158 @@ var fracClientSumOK : [Ref]real;
 var packedClientSumGreater0 : [Ref]bool;
 var fracClientSumGreater0 : [Ref]real;
 
-procedure PackClientSumOK(this:Ref);
+procedure PackClientSumOK(suCli:Ref, this:Ref);
 requires (packedClientSumOK[this] == false);
+requires sumClient[this] == suCli;
+// TODO add requires about parameters if needed
+requires (instanceof[suCli] == 1) ==> (fracSumOKProxySum[suCli] > 0.0) ;
+requires (instanceof[suCli] == 2) ==> (fracSumOKRealSum[suCli] > 0.0) ;
 
-procedure UnpackClientSumOK(this:Ref);
+procedure UnpackClientSumOK(suCli:Ref, this:Ref);
 requires packedClientSumOK[this];
 requires fracClientSumOK[this] > 0.0;
+ensures sumClient[this] == suCli;
+// TODO add requires about parameters if needed
+ensures (instanceof[suCli] == 1) ==> (fracSumOKProxySum[suCli] > 0.0) ;
+ensures (instanceof[suCli] == 2) ==> (fracSumOKRealSum[suCli] > 0.0) ;
 
-procedure PackClientSumGreater0(this:Ref);
+procedure PackClientSumGreater0(suCli:Ref, this:Ref);
 requires (packedClientSumGreater0[this] == false);
+requires sumClient[this] == suCli;
+// TODO add requires about parameters if needed
+requires (instanceof[suCli] == 1) ==> (fracSumGreater0ProxySum[suCli] > 0.0) ;
+requires (instanceof[suCli] == 2) ==> (fracSumGreater0RealSum[suCli] > 0.0) ;
 
-procedure UnpackClientSumGreater0(this:Ref);
+procedure UnpackClientSumGreater0(suCli:Ref, this:Ref);
 requires packedClientSumGreater0[this];
 requires fracClientSumGreater0[this] > 0.0;
+ensures sumClient[this] == suCli;
+// TODO add requires about parameters if needed
+ensures (instanceof[suCli] == 1) ==> (fracSumGreater0ProxySum[suCli] > 0.0) ;
+ensures (instanceof[suCli] == 2) ==> (fracSumGreater0RealSum[suCli] > 0.0) ;
 
-procedure ConstructClientSum(sum1:Ref, this:Ref);
+procedure ConstructClientSum(sum1:Ref, this:Ref)
+modifies sumClient, instanceof;
 ensures sumClient[this] == sum1;
+ensures (instanceof[sum1] == old(instanceof[sum1]));
+ensures (forall y:Ref :: ( (y!=sumClient[this]) ==> (instanceof[y] == old(instanceof[y]) ) ) );
+ensures (forall y:Ref :: ( (y!=this) ==> (sumClient[y] == old(sumClient[y]) ) ) );
+{
+	sumClient[this] := sum1;
+  instanceof[sumClient[this]] := instanceof[sum1];
+}
 
 procedure checkSumIsOK(this:Ref) returns (r:bool)
 requires (instanceof[sumClient[this]] == 1) ==> 
-	((fracSumOKProxySum[sumClient[this]] == 1.0) &&
+	((fracSumOKProxySum[sumClient[this]] > 0.0) &&
          packedSumOKProxySum[sumClient[this]] );
 requires (instanceof[sumClient[this]] == 2)==> 
-	((fracSumOKRealSum[sumClient[this]] == 1.0) &&
+	((fracSumOKRealSum[sumClient[this]] > 0.0) &&
+         packedSumOKRealSum[sumClient[this]]);
+ensures (instanceof[sumClient[this]] == 1) ==> 
+	((fracSumOKProxySum[sumClient[this]] > 0.0) &&
+         packedSumOKProxySum[sumClient[this]] );
+ensures (instanceof[sumClient[this]] == 2)==> 
+	((fracSumOKRealSum[sumClient[this]] > 0.0) &&
          packedSumOKRealSum[sumClient[this]]);
 {
 if (instanceof[sumClient[this]] == 1) {
-call r:=sumIsOKProxySum(sumClient[this]);
+call r := sumIsOKProxySum(sumClient[this]);
+} else if (instanceof[sumClient[this]] == 2){
+call r := sumIsOKRealSum(sumClient[this]);
 } else {
-call r:=sumIsOKRealSum(sumClient[this]);
+  // we cannot get into this branch
+  assume false;
 }
 
 }
 
 procedure checkSumGreater0(this:Ref) returns (r:bool)
 requires (instanceof[sumClient[this]] == 1) ==> 
-	((fracSumGreater0ProxySum[sumClient[this]] == 1.0) &&
+	((fracSumGreater0ProxySum[sumClient[this]] > 0.0) &&
          packedSumGreater0ProxySum[sumClient[this]] );
 requires (instanceof[sumClient[this]] == 2)==> 
-	((fracSumGreater0RealSum[sumClient[this]] == 1.0) &&
+	((fracSumGreater0RealSum[sumClient[this]] > 0.0) &&
+         packedSumGreater0RealSum[sumClient[this]]);
+ensures (instanceof[sumClient[this]] == 1) ==> 
+	((fracSumGreater0ProxySum[sumClient[this]] > 0.0) &&
+         packedSumGreater0ProxySum[sumClient[this]] );
+ensures (instanceof[sumClient[this]] == 2)==> 
+	((fracSumGreater0RealSum[sumClient[this]] > 0.0) &&
          packedSumGreater0RealSum[sumClient[this]]);
 {
 if (instanceof[sumClient[this]] == 1) {
 call r:=sumIsGreater0ProxySum(sumClient[this]);
-} else {
+} else if (instanceof[sumClient[this]] == 2) {
 call r:=sumIsGreater0RealSum(sumClient[this]);
+} else {
+  // we cannot get into this branch
+  assume false;
 }
 }
 
-procedure main(this:Ref) 
+procedure main1(this:Ref) 
+modifies packedSumOKProxySum, fracSumOKProxySum, 
+    packedClientSumOK, fracClientSumOK, sum, n,
+     realSum, sumClient, packedSumOKRealSum, fracSumOKRealSum, 
+     packedBasicFieldsRealSum, fracBasicFieldsRealSum, packedBasicFieldsProxySum,
+     fracBasicFieldsProxySum, instanceof;
 {
-var s,s2:Ref;
+var s:Ref;
 var client1, client2:Ref;
+var temp : real;
+var temp1 : real;
+var temp2 : bool;
+
+assume (forall y:Ref :: (fracSumOKProxySum[y] >= 0.0) );
+assume (forall y:Ref :: (fracSumGreater0ProxySum[y] >= 0.0) );
+
+assume (forall y:Ref :: (fracSumOKRealSum[y] >= 0.0) );
+assume (forall y:Ref :: (fracSumGreater0RealSum[y] >= 0.0) );
+
+call ConstructProxySum(5,s);
+packedBasicFieldsProxySum[s] := false;
+call PackBasicFieldsProxySum(sum[s], n[s], s);
+packedBasicFieldsProxySum[s] := true;
+fracBasicFieldsProxySum[s] := 1.0;
+instanceof[s] := 1;
+// could keep the if like below
+// but I instead simplified it
+call temp := calculateSumProxySum(s);
+call ConstructClientSum(s, client1);
+packedClientSumOK[client1] := false;
+call PackClientSumOK(s, client1);
+packedClientSumOK[client1] := true;
+fracClientSumOK[client1] := 1.0;
+
+call ConstructClientSum(s, client2);
+
+packedClientSumOK[client2] := false;
+call PackClientSumOK(s, client2);
+packedClientSumOK[client2] := true;
+fracClientSumOK[client2] := 1.0;
+
+call temp2 := checkSumIsOK(client1);
+
+//transfer from one object proposition to another
+packedBasicFieldsProxySum[s] := packedSumOKProxySum[s];
+
+call temp := calculateSumProxySum(s);
+
+call temp2 := checkSumIsOK(client2);
+}
+
+
+procedure main2(this:Ref) 
+modifies  sum,
+     packedSumGreater0ProxySum, fracSumGreater0ProxySum,
+     packedClientSumGreater0, fracClientSumGreater0, n,
+     realSum, sumClient, packedBasicFieldsRealSum, packedSumOKRealSum, fracSumOKRealSum,
+     fracBasicFieldsRealSum, packedBasicFieldsProxySum,
+     fracBasicFieldsProxySum, packedSumGreater0RealSum, fracSumGreater0RealSum,
+     instanceof;
+{
+var s2:Ref;
 var client3, client4:Ref;
 var temp : real;
 var temp1 : real;
@@ -71,75 +172,34 @@ assume (forall y:Ref :: (fracSumGreater0ProxySum[y] >= 0.0) );
 assume (forall y:Ref :: (fracSumOKRealSum[y] >= 0.0) );
 assume (forall y:Ref :: (fracSumGreater0RealSum[y] >= 0.0) );
 
-call ConstructProxySum(0,0,s);
-packedSumOKProxySum[s] := false;
-call PackSumOKProxySum(sum[s],n[s],s);
-packedSumOKProxySum[s] := true;
-fracSumOKProxySum[s] := 1.0;
-
-call ConstructClientSum(s, client1);
-packedClientSumOK[client1] := false;
-call PackClientSumOK(client1);
-packedClientSumOK[client1] := true;
-fracClientSumOK[client1] := 1.0;
-
-call ConstructClientSum(s, client2);
-packedClientSumOK[client2] := false;
-call PackClientSumOK(client2);
-packedClientSumOK[client2] := true;
-fracClientSumOK[client2] := 1.0;
-
-if (instanceof[s] == 1) {
-	call temp := calculateSumProxySum(5,s);
-} else {
-	call temp := calculateSumRealSum(5,s);
-}
-
-call temp2 := checkSumIsOK(client1);
-
-if (instanceof[s] == 1) {
-	call temp := calculateSumProxySum(5,s);
-} else {
-	call temp := calculateSumRealSum(5,s);
-}
-
-call temp2 := checkSumIsOK(client2);
-
-//------
-
-call ConstructProxySum(0,0,s2);
-packedSumGreater0ProxySum[s2] := false;
-call PackSumGreater0ProxySum(sum[s2],s2);
-packedSumGreater0ProxySum[s2] := true;
-fracSumGreater0ProxySum[s2] := 1.0;
+call ConstructProxySum(7,s2);
+packedBasicFieldsProxySum[s2] := false;
+call PackBasicFieldsProxySum(sum[s2], n[s2], s2);
+packedBasicFieldsProxySum[s2] := true;
+fracBasicFieldsProxySum[s2] := 1.0;
+instanceof[s2] := 1;
+call temp1 := addOneToSumProxySum(s2);
 
 call ConstructClientSum(s2, client3);
 packedClientSumGreater0[client3] := false;
-call PackClientSumGreater0(client3);
+call PackClientSumGreater0(s2, client3);
 packedClientSumGreater0[client3] := true;
 fracClientSumGreater0[client3] := 1.0;
 
 call ConstructClientSum(s2, client4);
 packedClientSumGreater0[client4] := false;
-call PackClientSumGreater0(client4);
+call PackClientSumGreater0(s2, client4);
 packedClientSumGreater0[client4] := true;
 fracClientSumGreater0[client4] := 1.0;
 
-if (instanceof[s2] == 1) {
-	call temp1 := calculateSumProxySum(7,s2);
-} else {
-	call temp1 := calculateSumRealSum(7,s2);
-}
-
 call temp2 := checkSumGreater0(client3);
 
-if (instanceof[s2] == 1) {
-	call temp1 := calculateSumProxySum(7,s2);
-} else {
-	call temp1 := calculateSumRealSum(7,s2);
-}
+//transfer from one object proposition to another
+packedBasicFieldsProxySum[s2] := packedSumGreater0ProxySum[s2];
+
+call temp1 := addOneToSumProxySum(s2);
+
 
 call temp2 := checkSumGreater0(client4);
-
 }
 
