college.bpl
@@ -1,3 +1,4 @@
+
 var collegeNumber :[Ref]int;
 var endowment : [Ref]int;
 
@@ -14,8 +15,8 @@ var packedCollegeFields : [Ref]bool;
 var fracCollegeFields : [Ref]real;
 
 procedure PackCollegeNumberField(c: int, this:Ref);
-requires (packedCollegeNumberField[this]==false) &&
- 	(collegeNumber[this] == c); 
+requires (packedCollegeNumberField[this]==false);
+requires (collegeNumber[this] == c); 
 
 procedure UnpackCollegeNumberField(c: int, this:Ref);
 requires packedCollegeNumberField[this];
@@ -23,92 +24,78 @@ requires fracCollegeNumberField[this] > 0.0;
 ensures	(collegeNumber[this] == c);
 
 procedure PackCollegeFields(c: int, this:Ref);
-requires (packedCollegeFields[this]==false) &&
- 	(collegeNumber[this] == c) && (endowment[this] == c*1000 - 5); 
+requires (packedCollegeFields[this]==false);
+requires (collegeNumber[this] == c);
+requires (endowment[this] == c*1000 - 5); 
 
-procedure UnpackCollegeFields(c:int, this:Ref);
+procedure UnpackCollegeFields(colNum:int, this:Ref);
 requires packedCollegeFields[this];
 requires fracCollegeFields[this] > 0.0;
-ensures	(collegeNumber[this] == c);
-ensures (endowment[this] == c*1000 - 5);
+ensures	(collegeNumber[this] == colNum);
+ensures (endowment[this] == colNum*1000 - 5);
 
-procedure PackCollegeFacilitiesMany(num:int, c:int, this:Ref);
+procedure PackCollegeFacilitiesMany(numFacilities:int, colNum:int, this:Ref);
 requires (packedCollegeFacilitiesMany[this] == false);
-//TODO all Pack procedures need to refer to frac also, 
-// not only to packed.
-requires (collegeNumber[this] == c) && (num >= 10 * c);
+requires (collegeNumber[this] == colNum);
+requires (numFacilities >= 10 * colNum);
 
-procedure UnpackCollegeFacilitiesMany(num:int, c:int, this:Ref);
+procedure UnpackCollegeFacilitiesMany(numFacilities:int, colNum:int, this:Ref);
 requires packedCollegeFacilitiesMany[this];
 requires fracCollegeFacilitiesMany[this] > 0.0;
-//TODO all Unpack procedures need to refer to frac also, 
-// not only to packed.
-ensures (collegeNumber[this] == c) && (num >= 10 * c);
+ensures (collegeNumber[this] == colNum);
+ensures	(numFacilities >= 10 * colNum);
 
-procedure PackCollegeFacilitiesFew(num:int, c:int, this:Ref);
+procedure PackCollegeFacilitiesFew(numFacilities:int, colNum:int, this:Ref);
 requires (packedCollegeFacilitiesFew[this] == false);
-requires (collegeNumber[this] == c) && (num <= 4 * c);
+requires (collegeNumber[this] == colNum);
+requires (numFacilities <= 4 * colNum);
 
-procedure UnpackCollegeFacilitiesFew(num:int, c:int, this:Ref);
+procedure UnpackCollegeFacilitiesFew(numFacilities:int, colNum:int, this:Ref);
 requires packedCollegeFacilitiesFew[this];
 requires fracCollegeFacilitiesFew[this] > 0.0;
-ensures (collegeNumber[this] == c) && (num <= 4 * c);
+ensures (collegeNumber[this] == colNum);
+ensures	(numFacilities <= 4 * colNum);
 
 procedure ConstructCollege(number:int, this:Ref) 
 modifies collegeNumber, endowment;
-ensures packedCollegeFields[this] &&
-	(fracCollegeFields[this] == 1.0);
+// Only for Construct we don't need the packed below. 
+// For the other procedures we do need to say about packed.
+//ensures packedCollegeFields[this];
+ensures (collegeNumber[this] == number);
+ensures (endowment[this] == (number *1000) - 5);
 // TODO need to put in statements about the parameters.
-// ensures this#1.0 CollegeFields()[number, (number*1000)-5]
+// ensures this#k CollegeFields()[number, (number*1000)-5]
 {
 	collegeNumber[this] := number;
 	endowment[this] := (number *1000) - 5;
 }
 
 procedure getCollegeNumber(this:Ref) returns (r:int)
-ensures packedCollegeNumberField[this] &&
-	(fracCollegeNumberField[this] == 1.0);
+requires packedCollegeNumberField[this];
+requires (fracCollegeNumberField[this] > 0.0);
+ensures packedCollegeNumberField[this];
+ensures	(fracCollegeNumberField[this] > 0.0);
 // TODO add statement about value of parameter 
-// ensures this#1.0 CollegeNumberField()[result]
+// ensures this#k CollegeNumberField()[result]
 {
 	r := collegeNumber[this];
 }
 
 // the method that calculates the extrinsic state
-procedure getNumberFacilities(int campusNumber) returns (r:Ref)
-requires packedCollegeNumberField[this] && 
-	(fracCollegeNumberField[this] == 1.0);
-//TODO have to say what are the current values of the parameters
-// requires this#1 CollegeNumberField(this.collegeNumber)
-ensures packedMultipleOf[r] &&
-	(fracMultipleOf[r] == 1.0);
-//ensures result#1 MultipleOf(this.collegeNumber)
+procedure getNumberFacilities(campNum:int, colNum:int, this:Ref) returns (r:int)
+modifies divider, value;
+  requires (collegeNumber[this] == colNum);
+  requires campNum > 0;
+  requires colNum > 0;
+  //TODO add an or of packed[] == false
+//requires packedCollegeNumberField[this]==false; 
+// I should add || packedCollegeFacilitiesMany == false 
+// || packedCollegeFacilitiesFew ==false
+//requires (fracCollegeNumberField[this] > 0.0);
+//TODO add ensures about the parameters
+ensures  r == colNum * campNum;
+ensures r> 0;
 {
-	call ConstructIntCell(collegeNumber[this] * campusNumber, r);
-	packedMultipleOf[r] := false;
-	call PackMultipleOf(collegeNumber[this], collegeNumber[this] * campusNumber, r)
-	packedMultipleOf[r] := true;
-	fracMultipleOf[r] := 1.0;
+	r := colNum * campNum;
 }
 
-procedure checkFewFacilities(num:int) returns (b:bool)
-requires packedCollegeFacilitiesFew[this] &&
-	(fracCollegeFacilitiesFew[this] == 1.0);
-//requires this#1 collegeFacilitiesFew(num)
-ensures packedCollegeFacilitiesFew[this] &&
-	(fracCollegeFacilitiesFew[this] == 1.0);
-//ensures this#1 collegeFacilitiesFew(num)
-{
-	r := (num <= 4 * collegeNumber[this]);
-}
-
-procedure checkManyFacilities(int num) returns (b:bool)
-requires packedCollegeFacilitiesMany[this] &&
-	(fracCollegeFacilitiesMany[this] == 1.0);
-//requires this#1 collegeFacilitiesMany(num)
-ensures packedCollegeFacilitiesMany[this] &&
-	(fracCollegeFacilitiesMany[this] == 1.0);
-//ensures this#1 collegeFacilitiesMany(num)
-{
-	r := (num >= 10 * collegeNumber[this]);
-}
