proxysum.bpl
@@ -1,3 +1,4 @@
+
 var packedSumOKProxySum: [Ref] bool;
 var fracSumOKProxySum: [Ref] real;
 var packedSumGreater0ProxySum: [Ref] bool;
@@ -7,58 +8,137 @@ var fracBasicFieldsProxySum: [Ref] real;
 
 var realSum: [Ref]Ref;
 
-procedure PackBasicFieldsProxySum(s1:real, n1:int, this:Ref);
+procedure PackBasicFieldsProxySum(su:real, n1:int, this:Ref);
 requires (packedBasicFieldsProxySum[this] == false);
-requires (sum[this] == s1) && (n[this]==n1);
+requires (n[this] == n1);
+requires (sum[this] == su);
+requires (n1 > 0);
 
-procedure UnpackBasicFieldsProxySum(s1:real, n1:int, this:Ref);
+procedure UnpackBasicFieldsProxySum(su:real, n1:int, this:Ref);
 requires packedBasicFieldsProxySum[this];
 requires fracBasicFieldsProxySum[this] > 0.0;
-ensures (sum[this] == s1) && (n[this]==n1);
+ensures	(n[this] == n1);
+ensures (sum[this] == su);
+ensures (n1 > 0);
 
-procedure PackSumOKProxySum(s1:real, n1:int, this:Ref);
+procedure PackSumOKProxySum(n1:int, this:Ref);
 requires (packedSumOKProxySum[this] == false);
-requires (sum[this] == s1) && (n[this]==n1) &&
-	( s1 == n1 * (n1+1) / 2 );
+requires (n[this] == n1);
+requires ( sum[this] == n1 * (n1+1) / 2 );
 
-procedure UnpackSumOKProxySum(s1:real, n1:int, this:Ref);
+procedure UnpackSumOKProxySum(n1:int, this:Ref);
 requires packedSumOKProxySum[this];
 requires fracSumOKProxySum[this] > 0.0;
-ensures (sum[this] == s1) && (n[this]==n1) &&
-	( s1 == n1 * (n1+1) / 2 );
+ensures	(n[this] == n1);
+ensures (sum[this] == (n1 * (n1+1) / 2));
 
 procedure PackSumGreater0ProxySum(s1:real, this:Ref);
 requires (packedSumGreater0ProxySum[this] == false);
-requires (sum[this] == s1) && (s1 > 0.0);
+requires (sum[this] == s1);
+requires (s1 > 0.0);
 
 procedure UnpackSumGreater0ProxySum(s1:real, this:Ref);
 requires packedSumGreater0ProxySum[this];
 requires fracSumGreater0ProxySum[this] > 0.0;
-ensures (sum[this] == s1) && (s1 > 0.0);
+ensures (sum[this] == s1);
+ensures	(s1 > 0.0);
 
-procedure ConstructProxySum(n1:int, s1:Ref, this:Ref);
+procedure ConstructProxySum(n1:int, this:Ref)
+modifies n, sum, realSum;
 ensures n[this] == n1;
-ensures sum[this] == s1;
+ensures sum[this] == 0.0;
+ensures (realSum[this] == null);
+{
+	n[this] := n1;
+	sum[this] := 0.0;
+	realSum[this] := null;
+}
 
-procedure calculateSumProxySum(n1:int, this:Ref)  returns (r:real)
-modifies n,sum;
+procedure calculateSumProxySum(this:Ref)  returns (r:real)
+modifies n, sum, packedSumOKRealSum, fracSumOKRealSum
+      , packedBasicFieldsRealSum, fracBasicFieldsRealSum, packedBasicFieldsProxySum,
+      packedSumOKProxySum, fracSumOKProxySum;
+requires packedBasicFieldsProxySum[this];
+requires (fracBasicFieldsProxySum[this] > 0.0);
+requires (realSum[this]!=null) ==> ( packedSumOKRealSum[realSum[this]] && (fracSumOKRealSum[realSum[this]] > 0.0));
+ensures packedSumOKProxySum[this];
+ensures	(fracSumOKProxySum[this] > 0.0);
 { 
+	var temp : real;
+  call UnpackBasicFieldsProxySum(sum[this], n[this], this);
+  packedBasicFieldsProxySum[this] := false;
+	if (realSum[this]==null) {
+		call ConstructRealSum(n[this], realSum[this]);
+		packedSumOKRealSum[realSum[this]] := false;
+		call PackSumOKRealSum(n[this], realSum[this]);
+		packedSumOKRealSum[realSum[this]] := true;
+		fracSumOKRealSum[realSum[this]] := 1.0;
+	}
+	  call temp := calculateSumRealSum(realSum[this]);
+  	sum[this] := temp;
+    n[this] := n[realSum[this] ];
+    
+    // transfer from one object proposition to another
+    packedSumOKProxySum[this] := packedBasicFieldsProxySum[this];
+    fracSumOKProxySum[this] := fracBasicFieldsProxySum[this];
+    call PackSumOKProxySum(n[this], this);
+    packedSumOKProxySum[this] := true;
+	  r := sum[this];
+}
+
+procedure addOneToSumProxySum(this:Ref) returns (r:real)
+modifies n, sum, packedSumOKRealSum, fracSumOKRealSum
+        , packedBasicFieldsRealSum, fracBasicFieldsRealSum,
+        packedSumGreater0RealSum, fracSumGreater0RealSum,
+        packedSumGreater0ProxySum, packedBasicFieldsProxySum,
+        fracSumGreater0ProxySum;
+requires packedBasicFieldsProxySum[this];
+//TODO should this be 1.0 or 0.0 , in all the requires here
+requires (fracBasicFieldsProxySum[this] == 1.0);
+requires (realSum[this]!=null) ==> ( packedBasicFieldsRealSum[realSum[this]] && (fracBasicFieldsRealSum[realSum[this]] > 0.0));
+ensures packedSumGreater0ProxySum[this];
+ensures (fracSumGreater0ProxySum[this] == 1.0);
+{
   var temp : real;
-n[this]:=n1;
-if (realSum[this]==null) {
-	call sumConstrRealSum(n[this], realSum[this]);
+	call UnpackBasicFieldsProxySum(sum[this], n[this], this);
+  packedBasicFieldsProxySum[this] := false;
+	if (realSum[this] == null) {
+		call ConstructRealSum(n[this], realSum[this]);
+		packedSumOKRealSum[realSum[this]] := false;
+		call PackSumOKRealSum(n[this], realSum[this]);
+		packedSumOKRealSum[realSum[this]] := true;
+		fracSumOKRealSum[realSum[this]] := 1.0;
+    // transfer one object proposition to another one
+    // which is less than this one
+    packedBasicFieldsRealSum[realSum[this]] := packedSumOKRealSum[realSum[this]];
+    fracBasicFieldsRealSum[realSum[this]] := fracSumOKRealSum[realSum[this]];
+	} 
+
+	call temp := addOneToSumRealSum(realSum[this]);
+  sum[this] := temp;
+  n[this] := n[realSum[this]];
+  // transfer from one object proposition to another
+  packedSumGreater0ProxySum[this] := packedBasicFieldsProxySum[this];
+  fracSumGreater0ProxySum[this] := fracBasicFieldsProxySum[this];
+  call PackSumGreater0ProxySum(sum[this], this);
+  packedSumGreater0ProxySum[this] := true;
+  r := sum[this];
 }
 
-	call temp := calculateSumRealSum(realSum[this]);
-  	sum[this]:=temp;
-	r:=sum[this];
-}
-
-procedure sumIsOKProxySum(this:Ref) returns (r:bool) {
-	r := (sum[this] == (n[this] * (n[this]+1) / 2));
+procedure sumIsOKProxySum(this:Ref) returns (r:bool)
+requires packedSumOKProxySum[this];
+requires (fracSumOKProxySum[this] > 0.0);
+ensures packedSumOKProxySum[this];
+ensures (fracSumOKProxySum[this] > 0.0); {
+	r := (sum[this] == (n[this] * (n[this]+1) / 2.0));
 }
 
 procedure sumIsGreater0ProxySum(this:Ref)  returns (r:bool)
+requires packedSumGreater0ProxySum[this];
+requires (fracSumGreater0ProxySum[this] > 0.0);
+ensures packedSumGreater0ProxySum[this];
+ensures (fracSumGreater0ProxySum[this] > 0.0);
 {
 	r:= (sum[this] > 0.0);
 }
+
