realsum.bpl
@@ -9,65 +9,130 @@ var fracSumGreater0RealSum: [Ref] real;
 const null: Ref;
 
 var n: [Ref]int;
+// sum can be considerent a dependent field on n
 var sum: [Ref]real;
 
-procedure PackBasicFieldsRealSum(s1:real, n1:int, this:Ref);
+procedure PackBasicFieldsRealSum(su:real, n1:int, this:Ref);
 requires (packedBasicFieldsRealSum[this] == false);
-requires (sum[this] == s1) && (n[this]==n1);
+requires (n[this]==n1);
+requires (sum[this] == su);
+requires n1 > 0;
 
-procedure UnpackBasicFieldsRealSum(s1:real, n1:int, this:Ref);
+procedure UnpackBasicFieldsRealSum(su:real, n1:int, this:Ref);
 requires packedBasicFieldsRealSum[this];
 requires fracBasicFieldsRealSum[this] > 0.0;
-ensures (sum[this] == s1) && (n[this]==n1);
+ensures	(n[this]==n1);
+ensures (sum[this] == su);
+ensures n1 > 0;
 
-procedure PackSumOKRealSum(s1:real, n1:int, this:Ref);
+procedure PackSumOKRealSum(n1:int, this:Ref);
 requires (packedSumOKRealSum[this] == false);
-requires (sum[this] == s1) && (n[this]==n1) &&
-	( s1 == n1 * (n1+1) / 2 );
+requires (n[this]==n1);
+requires n1 > 0;
+requires ( sum[this] == (n1 * (n1+1) / 2) );
 
-procedure UnpackSumOKRealSum(s1:real, n1:int, this:Ref);
+procedure UnpackSumOKRealSum(n1:int, this:Ref);
 requires packedSumOKRealSum[this];
 requires fracSumOKRealSum[this] > 0.0;
-ensures (sum[this] == s1) && (n[this]==n1) &&
-	( s1 == n1 * (n1+1) / 2 );
+ensures	(n[this]==n1);
+ensures n1 > 0;
+ensures	(sum[this] == (n1 * (n1+1) / 2) );
 
 procedure PackSumGreater0RealSum(s1:real, this:Ref);
 requires (packedSumGreater0RealSum[this] == false);
-requires (sum[this] == s1) && (s1 > 0.0);
+requires (sum[this] == s1);
+requires (s1 > 0.0);
 
 procedure UnpackSumGreater0RealSum(s1:real, this:Ref);
 requires packedSumGreater0RealSum[this];
 requires fracSumGreater0RealSum[this] > 0.0;
-ensures (sum[this] == s1) && (s1 > 0.0);
+ensures (sum[this] == s1);
+ensures	(s1 > 0.0);
 
-procedure ConstructRealSum(n1:int, s:Ref, this:Ref);
+procedure ConstructRealSum(n1:int, this:Ref)
+modifies n, sum, packedBasicFieldsRealSum, fracBasicFieldsRealSum, packedSumOKRealSum,
+        fracSumOKRealSum;
+requires n1 > 0;
 ensures n[this] == n1;
-ensures sum[this] == s;
-
-procedure calculateRealSum(n1:int, this:Ref) returns (r:real)
-modifies sum;
-requires packedBasicFieldsRealSum[this] && fracBasicFieldsRealSum[this]==1.0
-ensures packedSumOKRealSum[this] && fracSumOKRealSum[this]==1.0
+ensures sum[this] == (n1*(n1+1)/2);
+ensures (forall y:Ref :: ( (y!=this) ==> (n[y] == old(n[y]) ) ) );
 {
-	sum[this] := n1 * (n1 + 1) / 2;
+  	var temp:real;
+	n[this] := n1;
+  sum[this] := 0.0;
+  packedBasicFieldsRealSum[this] := false;
+  call PackBasicFieldsRealSum(0.0, n1, this);
+  packedBasicFieldsRealSum[this] := true;
+  fracBasicFieldsRealSum[this] := 1.0;
+	call temp := calculateRealSum(this);
+}
+
+procedure addOneToSumRealSum(this:Ref) returns (r:real)
+modifies n, sum, packedSumGreater0RealSum, packedSumOKRealSum,
+        fracSumOKRealSum, fracSumGreater0RealSum, packedBasicFieldsRealSum;
+requires packedBasicFieldsRealSum[this];
+requires (fracBasicFieldsRealSum[this] > 0.0);
+ensures packedSumGreater0RealSum[this];
+ensures (fracSumGreater0RealSum[this] > 0.0);
+ensures r > 0.0;
+{
+	var temp : real;
+	call temp := calculateRealSum(this);
+	sum[this] := temp + 1.0;
+  packedSumGreater0RealSum[this] := packedSumOKRealSum[this];
+  fracSumGreater0RealSum[this] := fracSumOKRealSum[this];
+  call PackSumGreater0RealSum(sum[this], this);
+  packedSumGreater0RealSum[this] := true;
+  r := sum[this];
+}
+
+procedure calculateSumRealSum(this:Ref)  returns (r:real)
+modifies sum, packedSumOKRealSum;
+requires packedSumOKRealSum[this];
+requires (fracSumOKRealSum[this] > 0.0);
+ensures r == (n[this]*(n[this]+1)/2);
+{ 
+  call UnpackSumOKRealSum(n[this], this);
+  packedSumOKRealSum[this] := false;
 	r := sum[this];
 }
 
-procedure calculateSumRealSum(n1:int, this:Ref)  returns (r:real)
-modifies n, sum;
-requires packedBasicFieldsRealSum[this] && fracBasicFieldsRealSum[this]==1.0
-ensures packedSumOKRealSum[this] && fracSumOKRealSum[this]==1.0
-
-{ 
-        n[this]:=n1;
-	call r:= calculateRealSum(n1, this);
+procedure calculateRealSum(this:Ref) returns (r:real)
+modifies sum, packedSumOKRealSum, fracSumOKRealSum, packedBasicFieldsRealSum;
+requires packedBasicFieldsRealSum[this];
+requires (fracBasicFieldsRealSum[this] > 0.0);
+ensures	(fracSumOKRealSum[this] == old(fracBasicFieldsRealSum[this]));
+ensures r > 0.0;
+ensures sum[this] == (n[this]*(n[this]+1)/2);
+ensures (packedSumOKRealSum[this] == false);
+//ensures (forall y:Ref :: ( (y!=this) ==> (fracSumOKRealSum[y] == old(fracSumOKRealSum[y]) ) ) );
+{
+  call UnpackBasicFieldsRealSum(sum[this], n[this], this);
+  packedBasicFieldsRealSum[this] := false;
+	sum[this] := n[this] * (n[this] + 1) / 2;
+	r := sum[this];
+  
+   // I transfer the fraction from one predicate to the other
+  packedSumOKRealSum[this] := packedBasicFieldsRealSum[this];
+  fracSumOKRealSum[this] := fracBasicFieldsRealSum[this];
 }
 
-procedure sumIsOKRealSum( this:Ref) returns (r:bool) {
+
+procedure sumIsOKRealSum( this:Ref) returns (r:bool) 
+requires packedSumOKRealSum[this];
+requires (fracSumOKRealSum[this] > 0.0);
+ensures packedSumOKRealSum[this];
+ensures (fracSumOKRealSum[this] > 0.0);
+{
 	r := (sum[this] == (n[this] * (n[this]+1) / 2));
 }
 
 procedure sumIsGreater0RealSum(this:Ref)  returns (r:bool)
+requires packedSumGreater0RealSum[this];
+requires (fracSumGreater0RealSum[this] > 0.0);
+ensures packedSumGreater0RealSum[this];
+ensures (fracSumGreater0RealSum[this] > 0.0);
 {
 	r:= (sum[this] > 0.0);
 }
+
